@prefix : <https://w3id.org/iot-tta#> .
@prefix cc: <http://creativecommons.org/ns#> .
@prefix owl: <http://www.w3.org/2002/07/owl#> .
@prefix rdf: <http://www.w3.org/1999/02/22-rdf-syntax-ns#> .
@prefix xml: <http://www.w3.org/XML/1998/namespace> .
@prefix xsd: <http://www.w3.org/2001/XMLSchema#> .
@prefix rdfs: <http://www.w3.org/2000/01/rdf-schema#> .
@prefix swrl: <http://www.w3.org/2003/11/swrl#> .
@prefix vann: <http://purl.org/vocab/vann/> .
@prefix voaf: <http://purl.org/vocommons/voaf#> .
@prefix swrla: <http://swrl.stanford.edu/ontologies/3.3/swrla.owl#> .
@prefix swrlb: <http://www.w3.org/2003/11/swrlb#> .
@prefix dcterms: <http://purl.org/dc/terms/> .
@base <https://w3id.org/iot-tta> .

<https://w3id.org/iot-tta> rdf:type owl:Ontology ;
                            owl:versionIRI <https://tudorliv.github.io/IoT-TTA/IIoT_v1.3.ttl> ;
                            cc:license <http://creativecommons.org/licenses/by/2.0/> ;
                            dcterms:contributor <https://orcid.org/0000-0002-0814-2615> ,
                                                <https://orcid.org/0000-0003-0702-6134> ,
                                                <https://orcid.org/0000-0003-1562-6922> ,
                                                <https://orcid.org/0000-0003-2392-7821> ;
                            dcterms:creator <https://orcid.org/0000-0001-6788-630X> ,
                                            <https://orcid.org/0000-0003-3562-0528> ;
                            dcterms:description " The Internet of Things taxonomy is extended with semantic ontologies for IoT layers, containing classes, properties, individuals, and rules specific to IoT technologies, tools, and applications."@en ;
                            dcterms:issued "2022-08-27"^^xsd:date ;
                            dcterms:modified "2022-09-02"^^xsd:date ,
                                             "2022-09-07"^^xsd:date ;
                            dcterms:title "Ontology for Internet of Things Technologies, Tools, and Applications"@en ;
                            vann:preferredNamespacePrefix "iot-tta" ;
                            vann:preferredNamespaceUri : ;
                            owl:versionInfo "Version 1.3" .

#################################################################
#    Annotation properties
#################################################################

###  http://creativecommons.org/ns#license
cc:license rdf:type owl:AnnotationProperty .


###  http://purl.org/dc/terms/contributor
dcterms:contributor rdf:type owl:AnnotationProperty .


###  http://purl.org/dc/terms/creator
dcterms:creator rdf:type owl:AnnotationProperty .


###  http://purl.org/dc/terms/description
dcterms:description rdf:type owl:AnnotationProperty .


###  http://purl.org/dc/terms/issued
dcterms:issued rdf:type owl:AnnotationProperty .


###  http://purl.org/dc/terms/modified
dcterms:modified rdf:type owl:AnnotationProperty .


###  http://purl.org/dc/terms/title
dcterms:title rdf:type owl:AnnotationProperty .


###  http://purl.org/vocab/vann/preferredNamespacePrefix
vann:preferredNamespacePrefix rdf:type owl:AnnotationProperty .


###  http://purl.org/vocab/vann/preferredNamespaceUri
vann:preferredNamespaceUri rdf:type owl:AnnotationProperty .


###  http://swrl.stanford.edu/ontologies/3.3/swrla.owl#isRuleEnabled
swrla:isRuleEnabled rdf:type owl:AnnotationProperty .


#################################################################
#    Object Properties
#################################################################

###  https://w3id.org/iot-tta#Dealing_with_sensitive_data
:Dealing_with_sensitive_data rdf:type owl:ObjectProperty ;
                             rdfs:domain :SCADA ;
                             rdfs:range :SCADA_solution ;
                             rdfs:comment "dealing_with_sensitive_data (Object property): SCADA solutions are proper practices for systems dealing with sensitive data"^^xsd:string ;
                             rdfs:label "dealing_with_sensitive_data"^^xsd:string .


###  https://w3id.org/iot-tta#DevelopEdgeSecurity
:DevelopEdgeSecurity rdf:type owl:ObjectProperty ;
                     rdfs:domain :Edge_application ;
                     rdfs:range :Blockchain_solution ;
                     rdfs:comment "developEdgeSecurity (Object property): develops solutions for edge applications using Blockchain capabilities"^^xsd:string ;
                     rdfs:label "developEdgeSecurity"^^xsd:string .


###  https://w3id.org/iot-tta#Lack_security_measure
:Lack_security_measure rdf:type owl:ObjectProperty ;
                       rdfs:domain :SCADA_common_protocol ;
                       rdfs:range :SCADA_problem ;
                       rdfs:comment "lack_security_measure (Object property): The SCADA common protocols such as Modbus and BACnet lack the built-in security measures"^^xsd:string ;
                       rdfs:label "lack_security_measure"^^xsd:string .


###  https://w3id.org/iot-tta#Protocols_were_layered
:Protocols_were_layered rdf:type owl:ObjectProperty ;
                        rdfs:domain :SCADA_common_protocol ;
                        rdfs:range :SCADA_today_protocol ;
                        rdfs:comment "protocols_were_layered (Object property): SCADA common protocols, such as Modbus and BACnet, were layered into Ethernet and TCP/IP"^^xsd:string ;
                        rdfs:label "protocols_were_layered"^^xsd:string .


###  https://w3id.org/iot-tta#SCADA_hasCapability
:SCADA_hasCapability rdf:type owl:ObjectProperty ;
                     rdfs:domain :SCADA ;
                     rdfs:range :SCADA_capability ;
                     rdfs:comment "scada_hasCapability (Object property): SCADA systems provide capabilities for industrial systems"^^xsd:string ;
                     rdfs:label "scada_hasCapability"^^xsd:string .


###  https://w3id.org/iot-tta#Support_communication
:Support_communication rdf:type owl:ObjectProperty ;
                       rdfs:domain :SCADA_today_protocol ;
                       rdfs:range :SCADA_capability ;
                       rdfs:comment "support_communication (Object property): SCADA systems perform communication with industrial systems in distributed architectures"^^xsd:string ;
                       rdfs:label "support_communication"^^xsd:string .


###  https://w3id.org/iot-tta#authentication
:authentication rdf:type owl:ObjectProperty ;
                rdfs:domain :MQTT ;
                rdfs:range :Asymmetric_public_keys ,
                           :JSON_Web_Token ;
                rdfs:comment "authentication (Object property): the MQTT and HTTP bridges use authentication with asymmetric public keys and JSON Web tokens"^^xsd:string ;
                rdfs:label "authentication"^^xsd:string .


###  https://w3id.org/iot-tta#best_Practices
:best_Practices rdf:type owl:ObjectProperty ;
                rdfs:domain :Edge_security ;
                rdfs:range :Edge_application ;
                rdfs:comment "best_Practices (Object property): defines the best practices for the edge security problems using Blockchain solutions"^^xsd:string ;
                rdfs:label "best_Practices"^^xsd:string .


###  https://w3id.org/iot-tta#challenge
:challenge rdf:type owl:ObjectProperty ;
           rdfs:domain :Blockchain ;
           rdfs:range :Blockchain_problem ;
           rdfs:comment "challenge (Object property): Blockchain technology comes with some challenges to implementation"^^xsd:string ;
           rdfs:label "challenge"^^xsd:string .


###  https://w3id.org/iot-tta#countermeasure
:countermeasure rdf:type owl:ObjectProperty ;
                rdfs:domain :SCADA_problem ;
                rdfs:range :SCADA_solution ;
                rdfs:comment "countermeasure (Object property): SCADA solutions represent countermeasure against threats generated by SCADA security problems"^^xsd:string ;
                rdfs:label "countermeasure"^^xsd:string .


###  https://w3id.org/iot-tta#data_transfer
:data_transfer rdf:type owl:ObjectProperty ;
               rdfs:domain :MQTT ;
               rdfs:range :Device ;
               rdfs:comment "data_transfer (Object property): an MQTT protocol transfers data provided by sensors"^^xsd:string ;
               rdfs:label "data_transfer"^^xsd:string .


###  https://w3id.org/iot-tta#flow_services
:flow_services rdf:type owl:ObjectProperty ;
               rdfs:domain :Particle_Photon ;
               rdfs:range :Subscriber ;
               rdfs:comment "flow_services: Object property that ensures the flows and services from Particle Photon to the subscriber (Thingspeak)"^^xsd:string ;
               rdfs:label "flow_services"^^xsd:string .


###  https://w3id.org/iot-tta#hasAlgorithm
:hasAlgorithm rdf:type owl:ObjectProperty ;
              rdfs:domain :Gateway ;
              rdfs:range :Analytics ,
                         :Machine_Learning ;
              rdfs:comment "hasAlgorithm (Object property): Gateway devices provide real-time analytics or machine learning algorithms, in edge computing"^^xsd:string ;
              rdfs:label "hasAlgorithm"^^xsd:string .


###  https://w3id.org/iot-tta#hasCapability
:hasCapability rdf:type owl:ObjectProperty ;
               rdfs:subPropertyOf owl:topObjectProperty ;
               rdfs:domain :Tool ;
               rdfs:range :BigData_capability ;
               rdfs:comment "hasCapability (Object property): tool that provides capabilities for big data processing in distributed systems"^^xsd:string ;
               rdfs:label "hasCapability"^^xsd:string .


###  https://w3id.org/iot-tta#hasElement
:hasElement rdf:type owl:ObjectProperty ;
            rdfs:domain :Andrew ;
            rdfs:range :Transducer ;
            rdfs:comment "hasElement (Object property): Sensor Andrew - sharing of transducers. There are two types of transducers: sensors and actuators."^^xsd:string ;
            rdfs:label "hasElement"^^xsd:string .


###  https://w3id.org/iot-tta#hasFunctionality
:hasFunctionality rdf:type owl:ObjectProperty ;
                  rdfs:domain :Data_center ;
                  rdfs:range :Cloud_service ;
                  rdfs:comment "hasFunctionality (Object property): a data center offers cloud services (as functionality)"^^xsd:string ;
                  rdfs:label "hasFunctionality"^^xsd:string .


###  https://w3id.org/iot-tta#hasProblem
:hasProblem rdf:type owl:ObjectProperty ;
            rdfs:domain :Blockchain ;
            rdfs:range :Blockchain_problem ;
            rdfs:comment "hasProblem (Object property): Blockchain technology has some problems"^^xsd:string ;
            rdfs:label "hasProblem"^^xsd:string .


###  https://w3id.org/iot-tta#hasSecurity_problem
:hasSecurity_problem rdf:type owl:ObjectProperty ;
                     rdfs:domain :Blockchain ;
                     rdfs:range :Blockchain_solution ;
                     rdfs:comment "hasSecurity_problem (Object property): security problems in Blockchain technology"^^xsd:string ;
                     rdfs:label "hasSecurity_problem"^^xsd:string .


###  https://w3id.org/iot-tta#hasService
:hasService rdf:type owl:ObjectProperty ,
                     owl:FunctionalProperty ;
            rdfs:domain :Data_center ;
            rdfs:range :Cloud_service ;
            rdfs:comment "hasService (Object property): specifies cloud services provided by data centers"^^xsd:string ;
            rdfs:label "hasService"^^xsd:string .


###  https://w3id.org/iot-tta#hasSolution
:hasSolution rdf:type owl:ObjectProperty ;
             rdfs:domain :Blockchain_problem ;
             rdfs:range :Blockchain_solution ;
             rdfs:comment "hasSolution (Object property): solutions for Blockchain problems"^^xsd:string ;
             rdfs:label "hasSolution"^^xsd:string .


###  https://w3id.org/iot-tta#hasTechnology
:hasTechnology rdf:type owl:ObjectProperty ;
               rdfs:domain :Edge_application ;
               rdfs:range :Edge_technology ;
               rdfs:comment "hasTechnology (Object property): the technology used in edge computing applications"^^xsd:string ;
               rdfs:label "hasTechnology"^^xsd:string .


###  https://w3id.org/iot-tta#hasTool
:hasTool rdf:type owl:ObjectProperty ;
         rdfs:domain :Technology ;
         rdfs:range :Tool ;
         rdfs:comment "hasTool (Object property): a tool used for the implementation of a technology"^^xsd:string ;
         rdfs:label "hasTool"^^xsd:string .


###  https://w3id.org/iot-tta#has_SecuritySolution
:has_SecuritySolution rdf:type owl:ObjectProperty ;
                      rdfs:domain :Edge_security ;
                      rdfs:range :Blockchain_solution ;
                      rdfs:comment "has_SecuritySolution (Object property): defines the best practices based on Blockchain solutions for edge security problems"^^xsd:string ;
                      rdfs:label "has_SecuritySolution"^^xsd:string .


###  https://w3id.org/iot-tta#heat
:heat rdf:type owl:ObjectProperty ;
      rdfs:domain :RTD_sensor ;
      rdfs:range :Industrial_oven ;
      rdfs:comment "heat (Object property): RTD sensors provide heat for some industrial ovens"^^xsd:string ;
      rdfs:label "heat"^^xsd:string .


###  https://w3id.org/iot-tta#isApplied
:isApplied rdf:type owl:ObjectProperty ;
           rdfs:domain :Tool ;
           rdfs:range :Computer_cluster ;
           rdfs:comment "isApplied (Object property): a tool used for computer clusters"^^xsd:string ;
           rdfs:label "isApplied"^^xsd:string .


###  https://w3id.org/iot-tta#isConnectedBy
:isConnectedBy rdf:type owl:ObjectProperty ;
               rdfs:domain :Processing_Board ;
               rdfs:range :Smart_Product ;
               rdfs:comment "isConnectedBy (Object property): modules with sensors or actuators connect processing boards with smart products"^^xsd:string ;
               rdfs:label "isConnectedBy"^^xsd:string .


###  https://w3id.org/iot-tta#isIdentified
:isIdentified rdf:type owl:ObjectProperty ;
              rdfs:domain :Passive_things ;
              rdfs:range :BLE ,
                         :NFC_tag ,
                         :Optical_tag ,
                         :RFID_tag ;
              rdfs:comment "isIdentified (Object property): passive things are identified by protocols such as NFC tags, optical tags, BLE, RFID tag, etc."^^xsd:string ;
              rdfs:label "isIdentified"^^xsd:string .


###  https://w3id.org/iot-tta#isManagedBy
:isManagedBy rdf:type owl:ObjectProperty ;
             rdfs:domain :Smart_Product ;
             rdfs:range :Programming_Language ,
                        :Web_Technology ;
             rdfs:comment "isManagedBy (Object property): Smart products are managed using Web technologies and software platforms."^^xsd:string ;
             rdfs:label "isManagedBy"^^xsd:string .


###  https://w3id.org/iot-tta#isPartOf
:isPartOf rdf:type owl:ObjectProperty ;
          rdfs:domain :PLC ,
                      :SCADA ;
          rdfs:range :ICS ;
          rdfs:comment "isPartOf (Object property):  PLC/SCADA is part of ICS (Industrial Control Systems)"^^xsd:string ;
          rdfs:label "isPartOf"^^xsd:string .


###  https://w3id.org/iot-tta#isProcessed
:isProcessed rdf:type owl:ObjectProperty ;
             rdfs:domain :BigData ;
             rdfs:range :BigData_capability ;
             rdfs:comment "isProcessed (Object property): the big data relies on distributed processing and storing, data analytics, and machine learning"^^xsd:string ;
             rdfs:label "isProcessed"^^xsd:string .


###  https://w3id.org/iot-tta#isRepresentationOf
:isRepresentationOf rdf:type owl:ObjectProperty ;
                    rdfs:domain :Digital_twin ;
                    rdfs:range :Smart_Product ;
                    rdfs:comment "isRepresentationOf (Object property): A digital twin from the cloud is a software representation of a smart product"^^xsd:string ;
                    rdfs:label "isRepresentationOf"^^xsd:string .


###  https://w3id.org/iot-tta#isToolFor
:isToolFor rdf:type owl:ObjectProperty ;
           rdfs:domain :Tool ;
           rdfs:range :Technology ;
           rdfs:comment "isToolFor (Object property): tool for distributed computing technologies"^^xsd:string ;
           rdfs:label "isToolFor"^^xsd:string .


###  https://w3id.org/iot-tta#isUsedBy
:isUsedBy rdf:type owl:ObjectProperty ;
          rdfs:domain :Tool ;
          rdfs:range :Technology ;
          rdfs:comment "isUsedBy (Object property): a tool used by a particular technology"^^xsd:string ;
          rdfs:label "isUsedBy"^^xsd:string .


###  https://w3id.org/iot-tta#login
:login rdf:type owl:ObjectProperty ;
       rdfs:domain :Mobile_node ;
       rdfs:range :Gateway ;
       rdfs:comment "login (Object property): In a wireless sensor network, a mobile node logins with a password using a gateway and Publish-Subscribe service."^^xsd:string ;
       rdfs:label "login"^^xsd:string .


###  https://w3id.org/iot-tta#manages
:manages rdf:type owl:ObjectProperty ;
         rdfs:domain :Gateway ;
         rdfs:range :Sensor_Actuator ;
         rdfs:comment "manages (Object property): Gateways manage the data from multiple devices and send them to the cloud"^^xsd:string ;
         rdfs:label "manages"^^xsd:string .


###  https://w3id.org/iot-tta#read
:read rdf:type owl:ObjectProperty ;
      rdfs:domain :Flow ;
      rdfs:range :Firmware ;
      rdfs:comment "read (Object property): A firmware program reads the D0 value of the 3V3 pin, in an application with a  Particle Photon that publishes messages using a Webhook."^^xsd:string ;
      rdfs:label "read"^^xsd:string .


###  https://w3id.org/iot-tta#regulationTemperature
:regulationTemperature rdf:type owl:ObjectProperty ;
                       rdfs:domain :RTD_sensor ;
                       rdfs:range :Industrial_oven ;
                       rdfs:comment "regulationTemperature (Object property): regulation of the RTD sensors’ temperature for an industrial oven"^^xsd:string ;
                       rdfs:label "regulationTemperature"^^xsd:string .


###  https://w3id.org/iot-tta#request
:request rdf:type owl:ObjectProperty ;
         rdfs:domain :Particle_cloud ;
         rdfs:range :Subscriber ;
         rdfs:comment "request (Object property): Particle cloud service will forward messages with values “1” and “0” to Thingspeak as a subscriber. A Webhook (a new HTTP request to Thingspeak) will result after passing values to the Particle cloud."^^xsd:string ;
         rdfs:label "request"^^xsd:string .


###  https://w3id.org/iot-tta#requires
:requires rdf:type owl:ObjectProperty ;
          rdfs:domain :BigData_app ;
          rdfs:range :BigData_capability ;
          rdfs:comment "requires (Object property): Applications with Big Data require Big data capabilities - distributed processing and storing, etc."^^xsd:string ;
          rdfs:label "requires"^^xsd:string .


###  https://w3id.org/iot-tta#send
:send rdf:type owl:ObjectProperty ;
      rdfs:domain :Firmware ;
      rdfs:range :Particle_cloud ;
      rdfs:comment "send (Object property): A firmware program that reads the D0 value every 30 seconds, calls the function Particle.publish() with one of the values “0” or “1” that is sent to the Particle cloud."^^xsd:string ;
      rdfs:label "send"^^xsd:string .


###  https://w3id.org/iot-tta#supporting_tool
:supporting_tool rdf:type owl:ObjectProperty ;
                 rdfs:domain :Edge_application ;
                 rdfs:range :Tool ;
                 rdfs:comment "supporting_tool (Object property): tools for edge computing applications"^^xsd:string ;
                 rdfs:label "supporting_tool"^^xsd:string .


###  https://w3id.org/iot-tta#threats_to_data_security
:threats_to_data_security rdf:type owl:ObjectProperty ;
                          rdfs:domain :SCADA ;
                          rdfs:range :SCADA_problem ;
                          rdfs:comment "threats_to_data_security (Object property): SCADA protocols require an adequate defense against data security threats"^^xsd:string ;
                          rdfs:label "threats_to_data_security"^^xsd:string .


###  https://w3id.org/iot-tta#useAlgorithm
:useAlgorithm rdf:type owl:ObjectProperty ;
              rdfs:subPropertyOf owl:topObjectProperty ;
              rdfs:domain :Data_center ;
              rdfs:range :Data_center ;
              rdfs:comment "useAlgorithm (Object property): algorithms used in data centers"^^xsd:string ;
              rdfs:label "useAlgorithm"^^xsd:string .


###  https://w3id.org/iot-tta#useProgramming
:useProgramming rdf:type owl:ObjectProperty ;
                rdfs:subPropertyOf owl:topObjectProperty ;
                rdfs:domain :Tool ;
                rdfs:range :Tool ;
                rdfs:comment "useProgramming (Object property): defines the programming model used by tools for computer clusters"^^xsd:string ;
                rdfs:label "useProgramming"^^xsd:string .


###  https://w3id.org/iot-tta#wire
:wire rdf:type owl:ObjectProperty ;
      rdfs:domain :Particle_Photon ;
      rdfs:range :Flow ;
      rdfs:comment "wire (Object property): When the wire of a Particle Photon is connected, the Photon will send the value “1”, but if the wire is disconnected, the Photon will send the value “0”."^^xsd:string ;
      rdfs:label "wire"^^xsd:string .


#################################################################
#    Data properties
#################################################################

###  https://w3id.org/iot-tta#FireFly_nodes
:FireFly_nodes rdf:type owl:DatatypeProperty ;
               rdfs:domain :Wireless_sensor_network ,
                           [ rdf:type owl:Restriction ;
                             owl:onProperty :FireFly_nodes ;
                             owl:someValuesFrom [ rdf:type rdfs:Datatype ;
                                                  owl:onDatatype xsd:integer ;
                                                  owl:withRestrictions ( [ xsd:minInclusive 20
                                                                         ]
                                                                         [ xsd:maxInclusive 32
                                                                         ]
                                                                       )
                                                ]
                           ] ;
               rdfs:range xsd:integer ;
               rdfs:comment "fireFly_nodes (Data property): in a FireFly wireless sensor network, each gateway is set to manage between 20 and 32 network nodes"^^xsd:string ;
               rdfs:label "fireFly_nodes"^^xsd:string .


###  https://w3id.org/iot-tta#MicroSD_card
:MicroSD_card rdf:type owl:DatatypeProperty ;
              rdfs:subPropertyOf owl:topDataProperty ;
              rdfs:domain :Raspberyy_Pi_4B ,
                          [ rdf:type owl:Restriction ;
                            owl:onProperty :MicroSD_card ;
                            owl:someValuesFrom [ rdf:type rdfs:Datatype ;
                                                 owl:onDatatype xsd:double ;
                                                 owl:withRestrictions ( [ xsd:minInclusive "8.0"^^xsd:double
                                                                        ]
                                                                      )
                                               ]
                          ] ;
              rdfs:range xsd:double ;
              rdfs:comment "microSD_card (Data property): setting up Raspberry Pi 4 Model B requires a microSD card with a capacity of at least 8GB"^^xsd:string ;
              rdfs:label "microSD_card"^^xsd:string .


###  https://w3id.org/iot-tta#Password_mobile_node
:Password_mobile_node rdf:type owl:DatatypeProperty ;
                      rdfs:domain :Wireless_sensor_network ,
                                  [ rdf:type owl:Restriction ;
                                    owl:onProperty :Password_mobile_node ;
                                    owl:hasValue "password"
                                  ] ;
                      rdfs:range xsd:string ;
                      rdfs:comment "password_mobile_node (Data property): in a FireFly wireless sensor network, a mobile node logins with a password of at most 100 bytes"^^xsd:string ;
                      rdfs:label "password_mobile_node"^^xsd:string .


###  https://w3id.org/iot-tta#Power_supply
:Power_supply rdf:type owl:DatatypeProperty ;
              rdfs:subPropertyOf owl:topDataProperty ;
              rdfs:domain :Raspberyy_Pi_4B ,
                          [ rdf:type owl:Restriction ;
                            owl:onProperty :Power_supply ;
                            owl:someValuesFrom [ rdf:type rdfs:Datatype ;
                                                 owl:onDatatype xsd:float ;
                                                 owl:withRestrictions ( [ xsd:minInclusive "3.0"^^xsd:float
                                                                        ]
                                                                      )
                                               ]
                          ] ;
              rdfs:range xsd:float ;
              rdfs:comment "power_supply (Data property): Setting up Raspberry Pi 4 Model B requires a power supply that provides at least 3.0 amps"^^xsd:string ;
              rdfs:label "power_supply"^^xsd:string .


###  https://w3id.org/iot-tta#RAM
:RAM rdf:type owl:DatatypeProperty ;
     rdfs:subPropertyOf owl:topDataProperty ;
     rdfs:domain :Raspberyy_Pi_4B ,
                 [ rdf:type owl:Restriction ;
                   owl:onProperty :RAM ;
                   owl:someValuesFrom [ rdf:type rdfs:Datatype ;
                                        owl:onDatatype xsd:integer ;
                                        owl:withRestrictions ( [ xsd:minInclusive 2
                                                               ]
                                                             )
                                      ]
                 ] ;
     rdfs:range xsd:integer ;
     rdfs:comment "ram (Data property): setting up Raspberry Pi 4 Model B requires at least 2GB RAM for use as a desktop computer"^^xsd:string ;
     rdfs:label "ram"^^xsd:string .


###  https://w3id.org/iot-tta#disconnect_timeout
:disconnect_timeout rdf:type owl:DatatypeProperty ;
                    rdfs:domain :Wireless_sensor_network ,
                                [ rdf:type owl:Restriction ;
                                  owl:onProperty :disconnect_timeout ;
                                  owl:someValuesFrom [ rdf:type rdfs:Datatype ;
                                                       owl:onDatatype xsd:integer ;
                                                       owl:withRestrictions ( [ xsd:maxInclusive 1
                                                                              ]
                                                                            )
                                                     ]
                                ] ;
                    rdfs:range xsd:integer ;
                    rdfs:comment "disconnect_timeout (Data property): in a FireFly wireless sensor network, the SAMPL messages require a disconnect timeout for replying to messages on the mobile device"^^xsd:string ;
                    rdfs:label "disconnect_timeout"^^xsd:string .


###  https://w3id.org/iot-tta#hasAccuracy
:hasAccuracy rdf:type owl:DatatypeProperty ;
             rdfs:domain :RTD_sensor ,
                         [ rdf:type owl:Restriction ;
                           owl:onProperty :hasAccuracy ;
                           owl:someValuesFrom [ rdf:type rdfs:Datatype ;
                                                owl:onDatatype xsd:float ;
                                                owl:withRestrictions ( [ xsd:minInclusive "0.1"^^xsd:float
                                                                       ]
                                                                       [ xsd:maxInclusive "1.0"^^xsd:float
                                                                       ]
                                                                     )
                                              ]
                         ] ;
             rdfs:range xsd:float ;
             rdfs:comment "hasAccuracy (Data property): the accuracy provided by RTD sensors is between 0.1 and 1 °C"^^xsd:string ;
             rdfs:label "hasAccuracy"^^xsd:string .


###  https://w3id.org/iot-tta#hasTemperatureRange
:hasTemperatureRange rdf:type owl:DatatypeProperty ;
                     rdfs:domain :Industrial_oven ,
                                 [ rdf:type owl:Restriction ;
                                   owl:onProperty :hasTemperatureRange ;
                                   owl:someValuesFrom [ rdf:type rdfs:Datatype ;
                                                        owl:onDatatype xsd:double ;
                                                        owl:withRestrictions ( [ xsd:minInclusive "500.0"^^xsd:double
                                                                               ]
                                                                               [ xsd:maxInclusive "510.0"^^xsd:double
                                                                               ]
                                                                             )
                                                      ]
                                 ] ;
                     rdfs:range xsd:double ;
                     rdfs:comment "hasTemperatureRange (Data property): an industrial oven for a production line that is heated to a very precise temperature range, between 500F and 510F"^^xsd:string ;
                     rdfs:label "hasTemperatureRange"^^xsd:string .


###  https://w3id.org/iot-tta#hasTimeLimit
:hasTimeLimit rdf:type owl:DatatypeProperty ;
              rdfs:domain :Firmware ,
                          [ rdf:type owl:Restriction ;
                            owl:onProperty :hasTimeLimit ;
                            owl:someValuesFrom [ rdf:type rdfs:Datatype ;
                                                 owl:onDatatype xsd:integer ;
                                                 owl:withRestrictions ( [ xsd:minInclusive 29
                                                                        ]
                                                                        [ xsd:maxInclusive 30
                                                                        ]
                                                                      )
                                               ]
                          ] ;
              rdfs:range xsd:integer ;
              rdfs:comment "hasTimeLimit (Data property): A firmware program reads the D0 value of the 3V3 pin every 30 seconds, for an application with a  Particle Photon with a single resistor that publishes messages using a Webhook."^^xsd:string ;
              rdfs:label "hasTimeLimit"^^xsd:string .


###  https://w3id.org/iot-tta#hasValueConnection
:hasValueConnection rdf:type owl:DatatypeProperty ;
                    rdfs:domain :Flow ,
                                [ rdf:type owl:Restriction ;
                                  owl:onProperty :hasValueConnection ;
                                  owl:someValuesFrom [ rdf:type rdfs:Datatype ;
                                                       owl:onDatatype xsd:integer ;
                                                       owl:withRestrictions ( [ xsd:minInclusive 0
                                                                              ]
                                                                              [ xsd:maxInclusive 1
                                                                              ]
                                                                            )
                                                     ]
                                ] ;
                    rdfs:range xsd:integer ;
                    rdfs:comment "hasValueConnection (Data property): if the wire of a Particle Photon is connected, the Photon sends the value “1”"^^xsd:string ;
                    rdfs:label "hasValueConnection"^^xsd:string .


###  https://w3id.org/iot-tta#languages_tools
:languages_tools rdf:type owl:DatatypeProperty ;
                 rdfs:domain :PLC ,
                             :Raspberry_Pi ,
                             [ rdf:type owl:Class ;
                               owl:unionOf ( [ rdf:type owl:Restriction ;
                                               owl:onProperty :languages_tools ;
                                               owl:hasValue "C"
                                             ]
                                             [ rdf:type owl:Restriction ;
                                               owl:onProperty :languages_tools ;
                                               owl:hasValue "C++"
                                             ]
                                             [ rdf:type owl:Restriction ;
                                               owl:onProperty :languages_tools ;
                                               owl:hasValue "Cosm"
                                             ]
                                             [ rdf:type owl:Restriction ;
                                               owl:onProperty :languages_tools ;
                                               owl:hasValue "Ladder Logic"
                                             ]
                                             [ rdf:type owl:Restriction ;
                                               owl:onProperty :languages_tools ;
                                               owl:hasValue "Nimbits"
                                             ]
                                             [ rdf:type owl:Restriction ;
                                               owl:onProperty :languages_tools ;
                                               owl:hasValue "Python"
                                             ]
                                             [ rdf:type owl:Restriction ;
                                               owl:onProperty :languages_tools ;
                                               owl:hasValue "Wyliodrin Studio"
                                             ]
                                           )
                             ] ;
                 rdfs:range xsd:string ;
                 rdfs:comment "languages_tools (Data property): tools and programming languages used by hardware platforms like PLC and Raspberry Pi"^^xsd:string ;
                 rdfs:label "languages_tools"^^xsd:string .


###  https://w3id.org/iot-tta#operating_system
:operating_system rdf:type owl:DatatypeProperty ;
                  rdfs:domain :Raspberry_Pi ,
                              [ rdf:type owl:Class ;
                                owl:unionOf ( [ rdf:type owl:Restriction ;
                                                owl:onProperty :operating_system ;
                                                owl:hasValue "Android"
                                              ]
                                              [ rdf:type owl:Restriction ;
                                                owl:onProperty :operating_system ;
                                                owl:hasValue "Linux"
                                              ]
                                              [ rdf:type owl:Restriction ;
                                                owl:onProperty :operating_system ;
                                                owl:hasValue "Mac"
                                              ]
                                              [ rdf:type owl:Restriction ;
                                                owl:onProperty :operating_system ;
                                                owl:hasValue "RaspberryPi"
                                              ]
                                              [ rdf:type owl:Restriction ;
                                                owl:onProperty :operating_system ;
                                                owl:hasValue "Raspbian"
                                              ]
                                              [ rdf:type owl:Restriction ;
                                                owl:onProperty :operating_system ;
                                                owl:hasValue "Windows"
                                              ]
                                            )
                              ] ;
                  rdfs:range xsd:string ;
                  rdfs:comment "operating_system (Data property): operating systems used by Raspberry Pi"^^xsd:string ;
                  rdfs:label "operating_system"^^xsd:string .


###  https://w3id.org/iot-tta#provideHeat
:provideHeat rdf:type owl:DatatypeProperty ;
             rdfs:domain :RTD_sensor ,
                         [ rdf:type owl:Restriction ;
                           owl:onProperty :provideHeat ;
                           owl:someValuesFrom [ rdf:type rdfs:Datatype ;
                                                owl:onDatatype xsd:double ;
                                                owl:withRestrictions ( [ xsd:minInclusive "-200.0"^^xsd:double
                                                                       ]
                                                                       [ xsd:maxInclusive "600.0"^^xsd:double
                                                                       ]
                                                                     )
                                              ]
                         ] ;
             rdfs:range xsd:double ;
             rdfs:comment "provideHeat (Data property): the RTD sensors provide heat between  -200 and 600 °C"^^xsd:string ;
             rdfs:label "provideHeat"^^xsd:string .


#################################################################
#    Classes
#################################################################

###  http://purl.org/vocommons/voaf#Vocabulary
voaf:Vocabulary rdf:type owl:Class .


###  https://w3id.org/iot-tta#AdaFruit
:AdaFruit rdf:type owl:Class ;
          rdfs:subClassOf :MQTT_streams ;
          rdfs:comment "Adafruit is a development board designed for Arduino, Raspberry Pi applications."^^xsd:string ;
          rdfs:label "AdaFruit"^^xsd:string .


###  https://w3id.org/iot-tta#Adapter
:Adapter rdf:type owl:Class ;
         rdfs:subClassOf :Gateway ;
         rdfs:comment "Adapters are gateways to external hardware platforms like Arduino and Raspberry PI."^^xsd:string ;
         rdfs:label "Adapter"^^xsd:string .


###  https://w3id.org/iot-tta#Algorithm
:Algorithm rdf:type owl:Class ;
           rdfs:subClassOf :Logic ;
           rdfs:comment "Algorithms for data analytics, data mining, neural networks, firmware, and tools for machine learning."^^xsd:string ;
           rdfs:label "Algorithm"^^xsd:string .


###  https://w3id.org/iot-tta#Analytics
:Analytics rdf:type owl:Class ;
           rdfs:subClassOf :Algorithm ;
           rdfs:comment "Tools for data analysis: Spark, Hortonworks, Cloudera, MapR, Watson IoT"^^xsd:string ;
           rdfs:label "Analytics"^^xsd:string .


###  https://w3id.org/iot-tta#Andrew
:Andrew rdf:type owl:Class ;
        rdfs:subClassOf :Sensor_Actuator ;
        rdfs:comment "Sensor Andrew - uniform access to heterogeneous devices; sharing of transducers; security and privacy, etc."^^xsd:string ;
        rdfs:label "Andrew"^^xsd:string .


###  https://w3id.org/iot-tta#Application
:Application rdf:type owl:Class ;
             rdfs:subClassOf :IoTLayers ;
             rdfs:comment "\"Application\" represents a layer of the IoT architecture. Application layer ontology includes terms and semantic rules regarding Blockchain technology, SCADA systems, and security issues in cloud and edge computing."^^xsd:string ;
             rdfs:label "Application"^^xsd:string .


###  https://w3id.org/iot-tta#Arduino
:Arduino rdf:type owl:Class ;
         rdfs:subClassOf :Microcontroller ;
         rdfs:comment "Arduino is a microcontroller based on the C++ language. Cosm and Nimbits are open platforms for storing sensor data on the Cloud."^^xsd:string ;
         rdfs:label "Arduino"^^xsd:string .


###  https://w3id.org/iot-tta#Asymmetric_public_keys
:Asymmetric_public_keys rdf:type owl:Class ;
                        rdfs:subClassOf :Cryptographic_system ;
                        rdfs:comment "The MQTT and HTTP bridges use authentication with asymmetric public key and JSON Web tokens, which increase device security."^^xsd:string ;
                        rdfs:label "Asymmetric_public_keys"^^xsd:string .


###  https://w3id.org/iot-tta#BLE
:BLE rdf:type owl:Class ;
     rdfs:subClassOf :Protocol ;
     rdfs:comment "BLE tags (Bluetooth Low Energy beacons) - protocols for small data exchanges are small Bluetooth hardware components that are used to locate people or objects."^^xsd:string ;
     rdfs:label "BLE"^^xsd:string .


###  https://w3id.org/iot-tta#BigData
:BigData rdf:type owl:Class ;
         rdfs:subClassOf :Technology ;
         rdfs:comment "The data stream from IoT systems is processed using cloud computing, big data, and artificial intelligence algorithms."^^xsd:string ;
         rdfs:label "BigData"^^xsd:string .


###  https://w3id.org/iot-tta#BigData_app
:BigData_app rdf:type owl:Class ;
             rdfs:subClassOf :Application ;
             rdfs:comment "Applications with Big Data - BigQuery, an enterprise data warehouse for large data that enables fast SQL queries"^^xsd:string ;
             rdfs:label "BigData_app"^^xsd:string .


###  https://w3id.org/iot-tta#BigData_capability
:BigData_capability rdf:type owl:Class ;
                    rdfs:subClassOf :BigData ;
                    rdfs:comment "Big data capabilities - distributed processing and storing, big data analytics, machine learning algorithms."^^xsd:string ;
                    rdfs:label "BigData_capability"^^xsd:string .


###  https://w3id.org/iot-tta#Blockchain
:Blockchain rdf:type owl:Class ;
            rdfs:subClassOf :Technology ;
            rdfs:comment "Blockchain is a promising technology for securing IoT data over a network. Blockchain has distributed capabilities for processing transactions and tracking assets in a business network."^^xsd:string ;
            rdfs:label "Blockchain"^^xsd:string .


###  https://w3id.org/iot-tta#Blockchain_app
:Blockchain_app rdf:type owl:Class ;
                rdfs:subClassOf :Application ;
                rdfs:comment "Blockchain can be used in IoT applications such as smart cities, e-health, agriculture, and IoT data processing."^^xsd:string ;
                rdfs:label "Blockchain_app"^^xsd:string .


###  https://w3id.org/iot-tta#Blockchain_problem
:Blockchain_problem rdf:type owl:Class ;
                    rdfs:subClassOf :Blockchain ;
                    rdfs:comment "Blockchain problems: (a) Blockchain algorithm requires energy that IoT devices may not manage; (b) IoT devices continue to stream data while Blockchain throughput is limited; (c) Almost impossible to identify illegal Blockchain transaction; (d) Blockchain’s transparency feature brings privacy challenges for IoT customer, etc."^^xsd:string ;
                    rdfs:label "Blockchain_problem"^^xsd:string .


###  https://w3id.org/iot-tta#Blockchain_security
:Blockchain_security rdf:type owl:Class ;
                     rdfs:subClassOf :Blockchain ;
                     rdfs:comment "Security for Blockchain is aimed at access control and securing communication between local IoT devices."^^xsd:string ;
                     rdfs:label "Blockchain_security"^^xsd:string .


###  https://w3id.org/iot-tta#Blockchain_solution
:Blockchain_solution rdf:type owl:Class ;
                     rdfs:subClassOf :Blockchain ;
                     rdfs:comment "Solutions for Blockchain problems - improving data privacy, reducing latency in sending data, and adjusting the deficiencies of the edge implementation"^^xsd:string ;
                     rdfs:label "Blockchain_solution"^^xsd:string .


###  https://w3id.org/iot-tta#C
:C rdf:type owl:Class ;
   rdfs:subClassOf :Programming_Language ;
   rdfs:comment "Embedded programming in C or C++ for IoT platforms like Arduino, Raspberry Pi, or Particle"^^xsd:string ;
   rdfs:label "C"^^xsd:string .


###  https://w3id.org/iot-tta#Capabilities
:Capabilities rdf:type owl:Class ;
              rdfs:subClassOf :IoTLayers ;
              rdfs:comment "\"Capabilities\" represents a layer of the IoT architecture and includes device and data management, security, privacy, and ethics."^^xsd:string ;
              rdfs:label "Capabilities"^^xsd:string .


###  https://w3id.org/iot-tta#Cloud_service
:Cloud_service rdf:type owl:Class ;
               rdfs:subClassOf :Support ;
               rdfs:comment "Cloud services perform communications between devices, data gathering and processing."^^xsd:string ;
               rdfs:label "Cloud_service"^^xsd:string .


###  https://w3id.org/iot-tta#Cloud_system
:Cloud_system rdf:type owl:Class ;
              rdfs:subClassOf :Support ;
              rdfs:comment "Cloud systems perform cloud computing. Instead of selling, cloud providers rent servers, storage space, databases, networks, software, analytics and business intelligence."^^xsd:string ;
              rdfs:label "Cloud_system"^^xsd:string .


###  https://w3id.org/iot-tta#Cloudera
:Cloudera rdf:type owl:Class ;
          rdfs:subClassOf :Tool ;
          rdfs:comment "Cloudera Data Platform (CDP) is a hybrid data platform for cloud computing, data analytics, and data management, offering performance, scalability, and security."^^xsd:string ;
          rdfs:label "Cloudera"^^xsd:string .


###  https://w3id.org/iot-tta#Cloudlet
:Cloudlet rdf:type owl:Class ;
          rdfs:subClassOf :Support ;
          rdfs:comment "Cloudlets are usually based on mini-center of servers with cloud services for mobile applications and edge computing. A cloudlet represents the middle level of a 3-level architecture: mobile device - cloudlet - cloud."^^xsd:string ;
          rdfs:label "Cloudlet"^^xsd:string .


###  https://w3id.org/iot-tta#Computer_architecture
:Computer_architecture rdf:type owl:Class ;
                       rdfs:subClassOf :Network ;
                       rdfs:comment "The Network class is defined as an aggregation of the three components: data transmission, control engineering, and computer architecture."^^xsd:string ;
                       rdfs:label "Computer_architecture"^^xsd:string .


###  https://w3id.org/iot-tta#Computer_cluster
:Computer_cluster rdf:type owl:Class ;
                  rdfs:subClassOf :Technology ;
                  rdfs:comment "A computer cluster is a set of computers that work together as a single system. Computer clusters have each node set to perform the same task, controlled and scheduled by software."^^xsd:string ;
                  rdfs:label "Computer_cluster"^^xsd:string .


###  https://w3id.org/iot-tta#Control_System
:Control_System rdf:type owl:Class ;
                rdfs:subClassOf :Purpose-built_Device ;
                rdfs:comment "Examples of industrial control systems based on IoT technology are manufacturing processes, power grids, etc."^^xsd:string ;
                rdfs:label "Control_System"^^xsd:string .


###  https://w3id.org/iot-tta#Control_engineering
:Control_engineering rdf:type owl:Class ;
                     rdfs:subClassOf :Network ;
                     rdfs:comment "The Network class is defined as an aggregation of the three components: data transmission, control engineering, and computer architecture."^^xsd:string ;
                     rdfs:label "Control_engineering"^^xsd:string .


###  https://w3id.org/iot-tta#Cryptographic_system
:Cryptographic_system rdf:type owl:Class ;
                      rdfs:subClassOf :Algorithm ;
                      rdfs:comment "A set of algorithms that convert plaintext to the ciphertext to encode or decode messages securely."^^xsd:string ;
                      rdfs:label "Cryptographic_system"^^xsd:string .


###  https://w3id.org/iot-tta#Data
:Data rdf:type owl:Class ;
      rdfs:subClassOf :Support ;
      rdfs:comment "Objects connected by sensors exchange data with other devices via the Internet."^^xsd:string ;
      rdfs:label "Data"^^xsd:string .


###  https://w3id.org/iot-tta#Data_analysis
:Data_analysis rdf:type owl:Class ;
               rdfs:subClassOf :Technology ;
               rdfs:comment "Data analysis is a process of inspecting, pre-processing, and modeling data for knowledge discovery, complex data aggregation, visualization, and reporting. Data mining is a particular data analysis technique focused on statistical algorithms for prediction, classification, clustering, etc."^^xsd:string ;
               rdfs:label "Data_analysis"^^xsd:string .


###  https://w3id.org/iot-tta#Data_center
:Data_center rdf:type owl:Class ;
             rdfs:subClassOf :Support ;
             rdfs:comment "A data center is a multicloud environment based on a network of computing, routers, switches, firewalls, storage systems, servers, and application-delivery controllers."^^xsd:string ;
             rdfs:label "Data_center"^^xsd:string .


###  https://w3id.org/iot-tta#Data_transmission
:Data_transmission rdf:type owl:Class ;
                   rdfs:subClassOf :Network ;
                   rdfs:comment "The Network class is defined as an aggregation of the three components: data transmission, control engineering, and computer architecture."^^xsd:string ;
                   rdfs:label "Data_transmission"^^xsd:string .


###  https://w3id.org/iot-tta#Deep_learning
:Deep_learning rdf:type owl:Class ;
               rdfs:subClassOf :Technology ;
               rdfs:comment "Deep learning is a branch of machine learning that relies on multilayer neural networks. Deep learning offers a refined and optimized method of computation, using hidden layers of a neural network that often learns from large amounts of data. Deep learning technologies - Theano, Tensor Flow, CNTK, MXnet, Caffe on Spark"^^xsd:string ;
               rdfs:label "Deep_learning"^^xsd:string .


###  https://w3id.org/iot-tta#Device
:Device rdf:type owl:Class ;
        rdfs:subClassOf :IoTLayers ;
        rdfs:comment "\"Device\" represents a layer of the IoT architecture. The device layer includes hardware platforms, connected products, technologies, tools, and functionalities."^^xsd:string ;
        rdfs:label "Device"^^xsd:string .


###  https://w3id.org/iot-tta#Digital
:Digital rdf:type owl:Class ;
         rdfs:subClassOf :Device ;
         rdfs:comment "Digital includes terms and tools about hardware platforms, logic, purpose-built devices, and smart products."^^xsd:string ;
         rdfs:label "Digital"^^xsd:string .


###  https://w3id.org/iot-tta#Digital_twin
:Digital_twin rdf:type owl:Class ;
              rdfs:subClassOf :Web_Technology ;
              rdfs:comment "A digital twin from the cloud can be associated with a device. The twin interacts with traditional browsers and with the backend device. The twin may be used to control or monitor the device."^^xsd:string ;
              rdfs:label "Digital_twin"^^xsd:string .


###  https://w3id.org/iot-tta#Distributed_operating_system
:Distributed_operating_system rdf:type owl:Class ;
                              rdfs:subClassOf :Support ;
                              rdfs:comment "A distributed operating system manages communication shared in a network of independent computers that possess their own memory unit and CPU. Ex: YARN, LOCUS, Mesos, etc."^^xsd:string ;
                              rdfs:label "Distributed_operating_system"^^xsd:string .


###  https://w3id.org/iot-tta#Distributed_processing
:Distributed_processing rdf:type owl:Class ;
                        rdfs:subClassOf :BigData_capability ;
                        rdfs:comment "Big data distributed processing - uploading significant volumes of data, data processing and analyzing, and distribution into the clustered database."^^xsd:string ;
                        rdfs:label "Distributed_processing"^^xsd:string .


###  https://w3id.org/iot-tta#Distributed_storage
:Distributed_storage rdf:type owl:Class ;
                     rdfs:subClassOf :BigData_capability ;
                     rdfs:comment "Big data distributed storage - stores and processes data on multiple machines, using services managed by cloud systems."^^xsd:string ;
                     rdfs:label "Distributed_storage"^^xsd:string .


###  https://w3id.org/iot-tta#Distributed_system
:Distributed_system rdf:type owl:Class ;
                    rdfs:subClassOf :Support ;
                    rdfs:comment "The support layer is represented by distributed systems known as “cloud systems” that perform communications between devices, data gathering and processing. A distributed system has components located on different  computers from the network that communicate by passing messages."^^xsd:string ;
                    rdfs:label "Distributed_system"^^xsd:string .


###  https://w3id.org/iot-tta#Django
:Django rdf:type owl:Class ;
        rdfs:subClassOf :Web_Technology ;
        owl:disjointWith :Node ;
        rdfs:comment "Software platforms (e.g., Python, Django, Node) and Web technologies are integrated with hardware components of the IoT systems. Django is a Python web framework used for the development of secure websites."^^xsd:string ;
        rdfs:label "Django"^^xsd:string .


###  https://w3id.org/iot-tta#Drone
:Drone rdf:type owl:Class ;
       rdfs:subClassOf :Purpose-built_Device ;
       rdfs:comment "Drones - flying IoT devices with full network connectivity capabilities."^^xsd:string ;
       rdfs:label "Drone"^^xsd:string .


###  https://w3id.org/iot-tta#Eddystone
:Eddystone rdf:type owl:Class ;
           rdfs:subClassOf :Smart_Product ;
           rdfs:comment "iBeacon from Apple and Eddystone from Google are portable electronic devices that use network protocols such as NFC, RFID, optical tags, or BLE as hardware transmitters."^^xsd:string ;
           rdfs:label "Eddystone"^^xsd:string .


###  https://w3id.org/iot-tta#Edge_application
:Edge_application rdf:type owl:Class ;
                  rdfs:subClassOf :Application ;
                  rdfs:comment "Applications based on edge computing - the term \"edge\" refers to any computational or network resource available between the data source and the cloud services."^^xsd:string ;
                  rdfs:label "Edge_application"^^xsd:string .


###  https://w3id.org/iot-tta#Edge_security
:Edge_security rdf:type owl:Class ;
               rdfs:subClassOf :Edge_technology ;
               rdfs:comment "The edge security must consider criteria based on memory size, computational cost, transmission speed, etc. Blockchain may offer security solutions."^^xsd:string ;
               rdfs:label "Edge_security"^^xsd:string .


###  https://w3id.org/iot-tta#Edge_technology
:Edge_technology rdf:type owl:Class ;
                 rdfs:subClassOf :Technology ;
                 rdfs:comment "The term edge refers to any computational or network resource available between the initial data source and the cloud services."^^xsd:string ;
                 rdfs:label "Edge_technology"^^xsd:string .


###  https://w3id.org/iot-tta#Electrical_Grids
:Electrical_Grids rdf:type owl:Class ;
                  rdfs:subClassOf :Purpose-built_Device ;
                  rdfs:comment "The administration of electrical grids once controlled by manual input and electrical relays have been replaced by industrial control systems (ICS)."^^xsd:string ;
                  rdfs:label "Electrical_Grids"^^xsd:string .


###  https://w3id.org/iot-tta#Ethics
:Ethics rdf:type owl:Class ;
        rdfs:subClassOf :Capabilities ;
        rdfs:comment "IoT systems should be ethics-compliant regarding the following key aspects: (a) human rights; (b) avoid subordination, manipulation, or stimulating addiction; (c) products and services aim to bring positive changes to the society, environment, persons, and economy."^^xsd:string ;
        rdfs:label "Ethics"^^xsd:string .


###  https://w3id.org/iot-tta#Factory_Equipment
:Factory_Equipment rdf:type owl:Class ;
                   rdfs:subClassOf :Purpose-built_Device ;
                   rdfs:comment "The administration of factory equipment is performed by the industrial control systems (ICS)."^^xsd:string ;
                   rdfs:label "Factory_Equipment"^^xsd:string .


###  https://w3id.org/iot-tta#Factory_Floor
:Factory_Floor rdf:type owl:Class ;
               rdfs:subClassOf :Purpose-built_Device ;
               rdfs:comment "The administration of factory floors is performed by the industrial control systems (ICS)."^^xsd:string ;
               rdfs:label "Factory_Floor"^^xsd:string .


###  https://w3id.org/iot-tta#Firmware
:Firmware rdf:type owl:Class ;
          rdfs:subClassOf :Algorithm ;
          rdfs:comment "In a Particle Photon application, a firmware program reads the value D0 of a pin, call the function Particle.publish() with one of the value “0” or “1” that is sent to the Particle cloud."^^xsd:string ;
          rdfs:label "Firmware"^^xsd:string .


###  https://w3id.org/iot-tta#Flow
:Flow rdf:type owl:Class ;
      rdfs:subClassOf :Particle_Photon ;
      rdfs:comment "Flow describes the Flow-Service-Quality semantics for a Particle Photon application that includes a Thingspeak subscriber, a WebHook, and a firmware program."^^xsd:string ;
      rdfs:label "Flow"^^xsd:string .


###  https://w3id.org/iot-tta#Gas_Meter
:Gas_Meter rdf:type owl:Class ;
           rdfs:subClassOf :Purpose-built_Device ;
           rdfs:comment "The administration of gas meters is performed by the industrial control systems (ICS)"^^xsd:string ;
           rdfs:label "Gas_Meter"^^xsd:string .


###  https://w3id.org/iot-tta#Gateway
:Gateway rdf:type owl:Class ;
         rdfs:subClassOf :Device ;
         rdfs:comment "Gateways process the data from multiple devices and send them to the cloud"^^xsd:string ;
         rdfs:label "Gateway"^^xsd:string .


###  https://w3id.org/iot-tta#Grid
:Grid rdf:type owl:Class ;
      rdfs:subClassOf :Support ;
      rdfs:comment "Grid computing is a form of distributed computing based on independent computers connected to a network by a network interface, such as Ethernet."^^xsd:string ;
      rdfs:label "Grid"^^xsd:string .


###  https://w3id.org/iot-tta#HAT
:HAT rdf:type owl:Class ;
     rdfs:subClassOf :Sensor_Actuator ;
     rdfs:comment "Modules that connect processing boards to computers and other objects"^^xsd:string ;
     rdfs:label "HAT"^^xsd:string .


###  https://w3id.org/iot-tta#HBase
:HBase rdf:type owl:Class ;
       rdfs:subClassOf :Tool ;
       rdfs:comment "HBase is a non-relational distributed database developed as part of Apache Hadoop. HBase runs on top of the Hadoop Distributed File System, providing capabilities like Bigtable."^^xsd:string ;
       rdfs:label "HBase"^^xsd:string .


###  https://w3id.org/iot-tta#HTTP
:HTTP rdf:type owl:Class ;
      rdfs:subClassOf :Protocol ;
      rdfs:comment "HTTP (Hypertext Transfer Protocol) is part of the Internet protocol suite, allows access to pages from Web servers. HTTP is an application layer protocol according to the OSI reference model."^^xsd:string ;
      rdfs:label "HTTP"^^xsd:string .


###  https://w3id.org/iot-tta#Hardware_Platform
:Hardware_Platform rdf:type owl:Class ;
                   rdfs:subClassOf :Digital ;
                   rdfs:comment "Examples of hardware platforms: a) microcontroller and computer platforms; b) HATs and Shields, modules that connect processing boards to computers and other objects."^^xsd:string ;
                   rdfs:label "Hardware_Platform"^^xsd:string .


###  https://w3id.org/iot-tta#Home_automation
:Home_automation rdf:type owl:Class ;
                 rdfs:subClassOf :Smart_Product ;
                 rdfs:comment "smart IoT systems for home - smart lighting, intelligent heating and cooling, motorized blinds, and automated windows and doors, etc."^^xsd:string ;
                 rdfs:label "Home_automation"^^xsd:string .


###  https://w3id.org/iot-tta#Hortonworks
:Hortonworks rdf:type owl:Class ;
             rdfs:subClassOf :Tool ;
             rdfs:comment "Hortonworks Data Platform (HDP) is a secure framework for distributed storage, processing of large, multi-source data sets, and data analysis."^^xsd:string ;
             rdfs:label "Hortonworks"^^xsd:string .


###  https://w3id.org/iot-tta#Hub
:Hub rdf:type owl:Class ;
     rdfs:subClassOf :Control_engineering ;
     rdfs:comment "The hub is a multi-port device that resends any received data packet to all of its ports except the one from which it received it."^^xsd:string ;
     rdfs:label "Hub"^^xsd:string .


###  https://w3id.org/iot-tta#ICS
:ICS rdf:type owl:Class ;
     rdfs:subClassOf :Industrial ;
     rdfs:comment "ICS (industrial control systems)"^^xsd:string ;
     rdfs:label "ICS"^^xsd:string .


###  https://w3id.org/iot-tta#IP
:IP rdf:type owl:Class ;
    rdfs:subClassOf :Protocol ;
    rdfs:comment "IP (Internet Protocol) is a protocol for transmitting data over the Internet. The data is retrieved and divided into datagrams (IP packets) by the transport layer, transmitted over the Internet, and then reassembled by the network layer."^^xsd:string ;
    rdfs:label "IP"^^xsd:string .


###  https://w3id.org/iot-tta#ISO_stack
:ISO_stack rdf:type owl:Class ;
           rdfs:subClassOf :Protocol ;
           rdfs:comment "ISO stack - protocols stack developed by the International Organization of Standardization (ISO) that works from the hardware physical layer to the software application layer."^^xsd:string ;
           rdfs:label "ISO_stack"^^xsd:string .


###  https://w3id.org/iot-tta#IaaS
:IaaS rdf:type owl:Class ;
      rdfs:subClassOf :Cloud_service ;
      rdfs:comment "IaaS (Infrastructure-as-a-Service) is a cloud service for sharing distributed virtualized resources. The cloud provider owns and operates the hardware and software components and the data center."^^xsd:string ;
      rdfs:label "IaaS"^^xsd:string .


###  https://w3id.org/iot-tta#Industrial
:Industrial rdf:type owl:Class ;
            rdfs:subClassOf :Control_System ;
            rdfs:comment "Examples of industrial control systems (ICS): manufacturing processes, power grids, oil and gas pipelines, etc."^^xsd:string ;
            rdfs:label "Industrial"^^xsd:string .


###  https://w3id.org/iot-tta#Industrial_oven
:Industrial_oven rdf:type owl:Class ;
                 rdfs:subClassOf :Industrial ;
                 rdfs:comment "Industrial ovens for a production line incorporate temperature sensors."^^xsd:string ;
                 rdfs:label "Industrial_oven"^^xsd:string .


###  https://w3id.org/iot-tta#Internet_standard
:Internet_standard rdf:type owl:Class ;
                   rdfs:subClassOf :Logic ;
                   rdfs:comment "Internet standards and tools"^^xsd:string ;
                   rdfs:label "Internet_standard"^^xsd:string .


###  https://w3id.org/iot-tta#IoTLayers
:IoTLayers rdf:type owl:Class ;
           rdfs:comment "IoT-TTA is a semantic ontology for the Internet of Things technologies, tools, and applications. IoT-TTA consists of a hierarchy of classes corresponding to the layers of a general IoT architecture: Device, Network, Support, Application, and Capabilities."^^xsd:string ;
           rdfs:label "IoTLayers"^^xsd:string .


###  https://w3id.org/iot-tta#JSON_Web_Token
:JSON_Web_Token rdf:type owl:Class ;
                rdfs:subClassOf :Internet_standard ;
                rdfs:comment "JSON Web Token is an Internet standard for creating data with optional signature and encryption."^^xsd:string ;
                rdfs:label "JSON_Web_Token"^^xsd:string .


###  https://w3id.org/iot-tta#Java
:Java rdf:type owl:Class ;
      rdfs:subClassOf :Programming_Language ;
      rdfs:comment "Java Programming for IoT Applications (e. g. IoT Java Application with Eclipse Kura)"^^xsd:string ;
      rdfs:label "Java"^^xsd:string .


###  https://w3id.org/iot-tta#Kafka
:Kafka rdf:type owl:Class ;
       rdfs:subClassOf :Distributed_system ;
       rdfs:comment "Kafka is a distributed log messaging system. Apache Kafka is a distributed event streaming platform used for data pipelines, data integration, and streaming analytics."^^xsd:string ;
       rdfs:label "Kafka"^^xsd:string .


###  https://w3id.org/iot-tta#LoRa
:LoRa rdf:type owl:Class ;
      rdfs:subClassOf :Sensor_Actuator ;
      rdfs:comment "LoRa (Long Range) performs the transmission with low power consumption, using the radio communication technique. LoRa devices have geolocation capabilities."^^xsd:string ;
      rdfs:label "LoRa"^^xsd:string .


###  https://w3id.org/iot-tta#LoRaWan
:LoRaWan rdf:type owl:Class ;
         rdfs:subClassOf :Sensor_Actuator ;
         rdfs:comment "LoRaWAN (protocol above LoRa) - LoRaWAN is a cloud-based Medium Access Control (MAC) layer protocol for managing communication between gateways and end-node devices."^^xsd:string ;
         rdfs:label "LoRaWan"^^xsd:string .


###  https://w3id.org/iot-tta#LoWPAN
:LoWPAN rdf:type owl:Class ;
        rdfs:subClassOf :Protocol ;
        rdfs:comment "The LoWPAN protocol belongs to the Internet layer and is extended from IP. It works on Low Power and Wireless Personal Area Network i.e., LoWPAN, and comprises an edge router and sensor nodes."^^xsd:string ;
        rdfs:label "LoWPAN"^^xsd:string .


###  https://w3id.org/iot-tta#Logic
:Logic rdf:type owl:Class ;
       rdfs:subClassOf :Digital ;
       owl:disjointWith :Smart_Product ;
       rdfs:comment "Logic class contains algorithms, Web technologies, tools, programming languages, and Internet protocols."^^xsd:string ;
       rdfs:label "Logic"^^xsd:string .


###  https://w3id.org/iot-tta#MQTT
:MQTT rdf:type owl:Class ;
      rdfs:subClassOf :Protocol ;
      rdfs:comment "MQTT (Message Queue Telemetry Transport) is a standard IoT protocol that transfers data provided by sensors and performs communications via satellite."^^xsd:string ;
      rdfs:label "MQTT"^^xsd:string .


###  https://w3id.org/iot-tta#MQTT_streams
:MQTT_streams rdf:type owl:Class ;
              rdfs:subClassOf :Data ;
              rdfs:comment "MQTT (Message Queue Telemetry Transport) is a data streaming standard based on publish-subscribe networks that can transport messages from devices to a server. Clients connect to a central server and publish certain data. Cloud services can automatically show MQTT streams."^^xsd:string ;
              rdfs:label "MQTT_streams"^^xsd:string .


###  https://w3id.org/iot-tta#Machine_Learning
:Machine_Learning rdf:type owl:Class ;
                  rdfs:subClassOf :Algorithm ;
                  rdfs:comment "The cloud ensures an efficient and scalable architecture for computation, data storage, and machine learning. Tools for machine learning: Mahout, Spark ML, TensorFlow, and Mllib."^^xsd:string ;
                  rdfs:label "Machine_Learning"^^xsd:string .


###  https://w3id.org/iot-tta#Machine_learning
:Machine_learning rdf:type owl:Class ;
                  rdfs:subClassOf :Application ;
                  rdfs:comment "Machine learning applications including artificial neural networks, data mining, genetic algorithms. Tools for machine learning: Mahout, Spark ML, Mllib, Tensor Flow, Theano, Python, Weka, R, Octave, etc."^^xsd:string ;
                  rdfs:label "Machine_learning"^^xsd:string .


###  https://w3id.org/iot-tta#Mahout
:Mahout rdf:type owl:Class ;
        rdfs:subClassOf :Machine_Learning ;
        rdfs:comment "Apache Mahout provides distributed machine learning algorithms. The Apache platforms use Hadoop or Spark. Mahout includes Java and Scala libraries and collections."^^xsd:string ;
        rdfs:label "Mahout"^^xsd:string .


###  https://w3id.org/iot-tta#Management
:Management rdf:type owl:Class ;
            rdfs:subClassOf :Capabilities ;
            rdfs:comment "Device and data management - Device management covers three operations: adding new devices, monitoring, and updating devices. The high-performance access to data from IoT applications can be maintained using Cloud Storage, an online storage service."^^xsd:string ;
            rdfs:label "Management"^^xsd:string .


###  https://w3id.org/iot-tta#MapR
:MapR rdf:type owl:Class ;
      rdfs:subClassOf :Tool ;
      rdfs:comment "MapReduce is a programming model for processing big data sets with a parallel, distributed algorithm on a cluster of computers. A MapReduce system has usually three operations: map, shuffle, and reduce. A popular open-source implementation is part of Apache Hadoop."^^xsd:string ;
      rdfs:label "MapR"^^xsd:string .


###  https://w3id.org/iot-tta#Mesos
:Mesos rdf:type owl:Class ;
       rdfs:subClassOf :Distributed_operating_system ;
       rdfs:comment "Mesos is a distributed operating system that runs on every machine. The Mesos kernel provides applications like Hadoop, Spark, Kafka and ensures resource management and scheduling in cloud environment."^^xsd:string ;
       rdfs:label "Mesos"^^xsd:string .


###  https://w3id.org/iot-tta#Microcontroller
:Microcontroller rdf:type owl:Class ;
                 rdfs:subClassOf :Hardware_Platform ;
                 rdfs:comment "CPU on a single chip; RAM, ROM, EEPROM, Timer, I/O, Serial Interface"^^xsd:string ;
                 rdfs:label "Microcontroller"^^xsd:string .


###  https://w3id.org/iot-tta#Microprocessor
:Microprocessor rdf:type owl:Class ;
                rdfs:subClassOf :Hardware_Platform ;
                rdfs:comment "CPU and several supporting chips; RAM, ROM, Input, Output, Serial Interface, Timers"^^xsd:string ;
                rdfs:label "Microprocessor"^^xsd:string .


###  https://w3id.org/iot-tta#Microprocessor_Platform
:Microprocessor_Platform rdf:type owl:Class ;
                         rdfs:subClassOf :Gateway ;
                         owl:disjointWith :Smartphone ;
                         rdfs:comment "Gateway devices (e.g. microprocessor platforms) enable a secure connection to the cloud and can do real-time analytics or machine learning"^^xsd:string ;
                         rdfs:label "Microprocessor_Platform"^^xsd:string .


###  https://w3id.org/iot-tta#Mllib
:Mllib rdf:type owl:Class ;
       rdfs:subClassOf :Machine_Learning ;
       rdfs:comment "MLlib (Machine Learning Library for Spark) contains algorithms such as classification, regression, clustering, and collaborative filtering."^^xsd:string ;
       rdfs:label "Mllib"^^xsd:string .


###  https://w3id.org/iot-tta#Mobile_node
:Mobile_node rdf:type owl:Class ;
             rdfs:subClassOf :Wireless_sensor_network ;
             rdfs:comment "In a wireless sensor network, a mobile node identifies nearby network nodes and logins with a password using the SAMPL protocol, gateway, and Publish-Subscribe service."^^xsd:string ;
             rdfs:label "Mobile_node"^^xsd:string .


###  https://w3id.org/iot-tta#NFC_tag
:NFC_tag rdf:type owl:Class ;
         rdfs:subClassOf :Protocol ;
         rdfs:comment "NFC tags (Near Field Communication limited to high-frequency) are protocols that identify passive things. NFC tags are passive, meaning they don't have any power source. They take power from the device that reads them, through magnetic induction."^^xsd:string ;
         rdfs:label "NFC_tag"^^xsd:string .


###  https://w3id.org/iot-tta#Network
:Network rdf:type owl:Class ;
         rdfs:subClassOf :IoTLayers ;
         rdfs:comment "\"Network\" represents a layer of the IoT architecture. The networking layer concerns data transmission among devices, the types of communications, and some network protocols used in IoT."^^xsd:string ;
         rdfs:label "Network"^^xsd:string .


###  https://w3id.org/iot-tta#Network_card
:Network_card rdf:type owl:Class ;
              rdfs:subClassOf :Computer_architecture ;
              rdfs:comment "The network card, also called \"network adapter\" or \"network interface card\", is a circuit that allows communication between the computer and the network (Internet, LAN)."^^xsd:string ;
              rdfs:label "Network_card"^^xsd:string .


###  https://w3id.org/iot-tta#NoSQL_Data
:NoSQL_Data rdf:type owl:Class ;
            rdfs:subClassOf :Data ;
            rdfs:comment "NoSQL database is a non-relational database. Types of NoSQL databases: document databases, key-value databases, wide-column stores, and graph databases. Ex. Azure Cosmos DB, Oracle NoSQL, MongoDB, Azure Cosmos DB, HBase databases, applications that use Hadoop, etc."^^xsd:string ;
            rdfs:label "NoSQL_Data"^^xsd:string .


###  https://w3id.org/iot-tta#Node
:Node rdf:type owl:Class ;
      rdfs:subClassOf :Web_Technology ;
      rdfs:comment "Software platforms (e.g., Python, Django, Node) and Web technologies are integrated with hardware components of the IoT systems. Node or NodeJS is a back-end Javascript runtime environment. Features: fast and real-time execution and good integration with IoT protocols."^^xsd:string ;
      rdfs:label "Node"^^xsd:string .


###  https://w3id.org/iot-tta#Oil_Pipeline_Control
:Oil_Pipeline_Control rdf:type owl:Class ;
                      rdfs:subClassOf :Purpose-built_Device ;
                      rdfs:comment "Sensors are embedded into purpose-built devices such as oil pipeline control systems."^^xsd:string ;
                      rdfs:label "Oil_Pipeline_Control"^^xsd:string .


###  https://w3id.org/iot-tta#Optical_tag
:Optical_tag rdf:type owl:Class ;
             rdfs:subClassOf :Protocol ;
             rdfs:comment "Identifying passive things can be performed using protocols such as optical tags, as hardware transmitters to nearby portable electronic devices."^^xsd:string ;
             rdfs:label "Optical_tag"^^xsd:string .


###  https://w3id.org/iot-tta#PAN
:PAN rdf:type owl:Class ;
     rdfs:subClassOf :Protocol ;
     rdfs:comment "PAN (Personal Area Network) is a network protocol that ensures the connection between devices within a radius of 10 meters. A PAN usually involves a PC, phone, personal digital assistant, tablet, printer, speakers, video game consoles, etc."^^xsd:string ;
     rdfs:label "PAN"^^xsd:string .


###  https://w3id.org/iot-tta#PLC
:PLC rdf:type owl:Class ;
     rdfs:subClassOf :Hardware_Platform ;
     rdfs:comment "PLC (Programmable Logic Controller) is a ruggedized computer. Features: valves, sensors, motors. PLC programming languages: Ladder Logic, Function Block Diagram, Sequential Function Chart; Connection with SCADA"^^xsd:string ;
     rdfs:label "PLC"^^xsd:string .


###  https://w3id.org/iot-tta#PaaS
:PaaS rdf:type owl:Class ;
      rdfs:subClassOf :Cloud_service ;
      rdfs:comment "PaaS (Platform-as-a-Service) is a cloud service that provides a virtual environment. PaaS provides the infrastructure and middleware components for developing and managing mobile and web applications in the cloud."^^xsd:string ;
      rdfs:label "PaaS"^^xsd:string .


###  https://w3id.org/iot-tta#Particle_Photon
:Particle_Photon rdf:type owl:Class ;
                 rdfs:subClassOf :Microcontroller ;
                 rdfs:comment "A Particle Photon application used for highlighting the Flow-Service-Quality semantics"^^xsd:string ;
                 rdfs:label "Particle_Photon"^^xsd:string .


###  https://w3id.org/iot-tta#Particle_cloud
:Particle_cloud rdf:type owl:Class ;
                rdfs:subClassOf :Particle_Photon ;
                rdfs:comment "Particle cloud describes the Flow-Service-Quality semantics for a Particle Photon application using the properties \"wire\", \"read\", \"send\", \"request\" and constraints based on \"hasTimeLimit\" and \"hasValueConnection\"."^^xsd:string ;
                rdfs:label "Particle_cloud"^^xsd:string .


###  https://w3id.org/iot-tta#Passive_things
:Passive_things rdf:type owl:Class ;
                rdfs:subClassOf :Smart_Product ;
                rdfs:comment "“Passive things” have sensors that do not require external power, they just react to inputs from their environment."^^xsd:string ;
                rdfs:label "Passive_things"^^xsd:string .


###  https://w3id.org/iot-tta#Peer-to-peer_system
:Peer-to-peer_system rdf:type owl:Class ;
                     rdfs:subClassOf :Support ;
                     rdfs:comment "A peer-to-peer system is a computer network that enables the sharing of network resources, computational power, and data storage, in an equal way between peers."^^xsd:string ;
                     rdfs:label "Peer-to-peer_system"^^xsd:string .


###  https://w3id.org/iot-tta#Privacy
:Privacy rdf:type owl:Class ;
         rdfs:subClassOf :Capabilities ;
         rdfs:comment "Privacy and data protection throughout their use and processing personal data"^^xsd:string ;
         rdfs:label "Privacy"^^xsd:string .


###  https://w3id.org/iot-tta#Processing_Board
:Processing_Board rdf:type owl:Class ;
                  rdfs:subClassOf :Sensor_Actuator ;
                  rdfs:comment "The processing board is an IoT board with a processor, memory (MicroSD, RAM), low-level IO, multimedia, inputs, connectivity, and power (usually USB connectors, headers, etc)."^^xsd:string ;
                  rdfs:label "Processing_Board"^^xsd:string .


###  https://w3id.org/iot-tta#Programming_Language
:Programming_Language rdf:type owl:Class ;
                      rdfs:subClassOf :Logic ;
                      rdfs:comment "IoT devices use certain programming languages to process and control data transfer (e.g. Raspberry Pi, Programmable Logic Controller, C, Java, Python)."^^xsd:string ;
                      rdfs:label "Programming_Language"^^xsd:string .


###  https://w3id.org/iot-tta#Protocol
:Protocol rdf:type owl:Class ;
          rdfs:subClassOf :Network ;
          rdfs:comment "A network protocol is a communication protocol implemented on a computer network or telecommunications network. Network protocols form protocol layers corresponding to OSI levels."^^xsd:string ;
          rdfs:label "Protocol"^^xsd:string .


###  https://w3id.org/iot-tta#Purpose-built_Device
:Purpose-built_Device rdf:type owl:Class ;
                      rdfs:subClassOf :Digital ;
                      rdfs:comment "Sensors are usually incorporated into connected objects or purpose-built devices such as components of a city’s infrastructure, controllers for factory equipment, oil pipeline control, etc."^^xsd:string ;
                      rdfs:label "Purpose-built_Device"^^xsd:string .


###  https://w3id.org/iot-tta#Python
:Python rdf:type owl:Class ;
        rdfs:subClassOf :Programming_Language ;
        rdfs:comment "Python programming for IoT systems uses libraries/packages such as numpy,  request, paho.mqtt.client, Countly, matplotlib, etc."^^xsd:string ;
        rdfs:label "Python"^^xsd:string .


###  https://w3id.org/iot-tta#RFID_tag
:RFID_tag rdf:type owl:Class ;
          rdfs:subClassOf :Protocol ;
          rdfs:comment "RFID tags (Radio Frequency Identification) are used as hardware transmitters to nearby portable electronic devices, for identifying passive things."^^xsd:string ;
          rdfs:label "RFID_tag"^^xsd:string .


###  https://w3id.org/iot-tta#RTD_sensor
:RTD_sensor rdf:type owl:Class ;
            rdfs:subClassOf :Sensor_Actuator ;
            rdfs:comment "RTD sensors of an industrial oven."^^xsd:string ;
            rdfs:label "RTD_sensor"^^xsd:string .


###  https://w3id.org/iot-tta#Raspberry_Pi
:Raspberry_Pi rdf:type owl:Class ;
              rdfs:subClassOf :Microcontroller ;
              rdfs:comment "Raspberry Pi uses operating systems such as Raspberry Pi OS, Raspbian, some versions of Linux, or Windows 10 IoT Core. Tools and programming languages: GPIO (general-purpose input/output) pins; PWM - Pulse-Width Modulation, Python, C/C++, Wyliodrin Studio"^^xsd:string ;
              rdfs:label "Raspberry_Pi"^^xsd:string .


###  https://w3id.org/iot-tta#Raspberyy_Pi_4B
:Raspberyy_Pi_4B rdf:type owl:Class ;
                 rdfs:subClassOf :Raspberry_Pi ;
                 rdfs:comment "Raspberry Pi uses operating systems like Linux, Raspbian (a Debian GNU/Linux), Raspberry Pi OS Lite, etc. Features: GPIO (general-purpose input/output) pins, PWM - Pulse-Width Modulation, programming languages and tools: GPIO with Scratch, Python, C/C++, Processing, Wyliodrin Studio, etc."^^xsd:string ;
                 rdfs:label "Raspberyy_Pi_4B"^^xsd:string .


###  https://w3id.org/iot-tta#Router
:Router rdf:type owl:Class ;
        rdfs:subClassOf :Control_engineering ;
        rdfs:comment "A router connects two or more computer networks using packet switching. These networks can be wired or wireless. A wireless router exchanges information between the network and the Internet using radio signals."^^xsd:string ;
        rdfs:label "Router"^^xsd:string .


###  https://w3id.org/iot-tta#SAMPL
:SAMPL rdf:type owl:Class ;
       rdfs:subClassOf :Protocol ;
       rdfs:comment "SAMPL is a compact network layer that operates on top of a low-power CSMA/CA-based MAC protocol. SAMPL operates as part of the sensor Andrew project at Carnegie Mellon University and FireFly wireless sensor networks."^^xsd:string ;
       rdfs:label "SAMPL"^^xsd:string .


###  https://w3id.org/iot-tta#SCADA
:SCADA rdf:type owl:Class ;
       rdfs:subClassOf :Hardware_Platform ;
       rdfs:comment "SCADA (Supervisory Control and Data Acquisition) is a control system comprising sensors, PLC (Programmable Logic Controllers), networked data communications, GUI for supervision of processes, and computers."^^xsd:string ;
       rdfs:label "SCADA"^^xsd:string .


###  https://w3id.org/iot-tta#SCADA_capability
:SCADA_capability rdf:type owl:Class ;
                  rdfs:subClassOf :SCADA ;
                  rdfs:comment "SCADA is used to centrally manage and monitor the various complex systems in an industrial setting. SCADA and ICS sensors make up the complex distributed industrial computing architecture."^^xsd:string ;
                  rdfs:label "SCADA_capability"^^xsd:string .


###  https://w3id.org/iot-tta#SCADA_common_protocol
:SCADA_common_protocol rdf:type owl:Class ;
                       rdfs:subClassOf :SCADA ;
                       rdfs:comment "The common protocols on which SCADA systems operate and transfer data are Modbus and BACnet."^^xsd:string ;
                       rdfs:label "SCADA_common_protocol"^^xsd:string .


###  https://w3id.org/iot-tta#SCADA_demand
:SCADA_demand rdf:type owl:Class ;
              rdfs:subClassOf :SCADA ;
              rdfs:comment "For SCADA systems, the demand for remote management and monitoring increased."^^xsd:string ;
              rdfs:label "SCADA_demand"^^xsd:string .


###  https://w3id.org/iot-tta#SCADA_problem
:SCADA_problem rdf:type owl:Class ;
               rdfs:subClassOf :SCADA ;
               rdfs:comment "The SCADA common protocols such as Modbus and BACnet lack the built-in security measures required to adequately defend against new threats directed at critical infrastructure."^^xsd:string ;
               rdfs:label "SCADA_problem"^^xsd:string .


###  https://w3id.org/iot-tta#SCADA_solution
:SCADA_solution rdf:type owl:Class ;
                rdfs:subClassOf :SCADA ;
                rdfs:comment "Insecure SCADA protocols were layered into Ethernet and TCP/IP to support long-distance communication."^^xsd:string ;
                rdfs:label "SCADA_solution"^^xsd:string .


###  https://w3id.org/iot-tta#SCADA_today_protocol
:SCADA_today_protocol rdf:type owl:Class ;
                      rdfs:subClassOf :SCADA ;
                      rdfs:comment "Ethernet and TCP/IP protocols are still used today by SCADA around the world."^^xsd:string ;
                      rdfs:label "SCADA_today_protocol"^^xsd:string .


###  https://w3id.org/iot-tta#SOA
:SOA rdf:type owl:Class ;
     rdfs:subClassOf :Application ;
     rdfs:comment "Applications based on the Service-Oriented Architecture (SOA)"^^xsd:string ;
     rdfs:label "SOA"^^xsd:string .


###  https://w3id.org/iot-tta#SaaS
:SaaS rdf:type owl:Class ;
      rdfs:subClassOf :Cloud_service ;
      rdfs:comment "SaaS (Software-as-a-Service) is a cloud service that supports running end-user applications. The cloud service provider develops and maintains software for cloud applications and makes the software available to its customers over the Internet."^^xsd:string ;
      rdfs:label "SaaS"^^xsd:string .


###  https://w3id.org/iot-tta#Satellite
:Satellite rdf:type owl:Class ;
           rdfs:subClassOf :Hardware_Platform ;
           rdfs:comment "MQTT performs communications via satellite"^^xsd:string ;
           rdfs:label "Satellite"^^xsd:string .


###  https://w3id.org/iot-tta#Security
:Security rdf:type owl:Class ;
          rdfs:subClassOf :Capabilities ;
          rdfs:comment "The security concerns for the IoT systems refer to denial-of-service (DoS) attacks through concurrent requests, weak protection credentials, insecure communication between devices, recovery, data backup during a system interruption, limited network visibility, etc."^^xsd:string ;
          rdfs:label "Security"^^xsd:string .


###  https://w3id.org/iot-tta#Sensor_Actuator
:Sensor_Actuator rdf:type owl:Class ;
                 rdfs:subClassOf :Device ;
                 rdfs:comment "The modules with sensors or actuators connect processing boards to computers and other devices. Unlike simple sensors, actuators can make changes in the environment."^^xsd:string ;
                 rdfs:label "Sensor_Actuator"^^xsd:string .


###  https://w3id.org/iot-tta#Shield
:Shield rdf:type owl:Class ;
        rdfs:subClassOf :Sensor_Actuator ;
        rdfs:comment "Modules that connect processing boards to computers and other objects"^^xsd:string ;
        rdfs:label "Shield"^^xsd:string .


###  https://w3id.org/iot-tta#Smart_Product
:Smart_Product rdf:type owl:Class ;
               rdfs:subClassOf :Digital ;
               rdfs:comment "Smart products are controlled and managed using Web technologies and software platforms."^^xsd:string ;
               rdfs:label "Smart_Product"^^xsd:string .


###  https://w3id.org/iot-tta#Smartphone
:Smartphone rdf:type owl:Class ;
            rdfs:subClassOf :Gateway ;
            rdfs:comment "Smartphones are gateway devices that enable data connectivity through their set of sensors: GPS, biometrics, Bluetooth, heart rate monitor, ECG, barcode readers, etc."^^xsd:string ;
            rdfs:label "Smartphone"^^xsd:string .


###  https://w3id.org/iot-tta#Spark
:Spark rdf:type owl:Class ;
       rdfs:subClassOf :Machine_Learning ,
                       :Tool ;
       rdfs:comment "Apache Spark is part of the Hadoop system. Spark allows big data processing and building machine learning models such as regression, classification, clustering, and recommendation systems in a distributed processing environment."^^xsd:string ;
       rdfs:label "Spark"^^xsd:string .


###  https://w3id.org/iot-tta#Subscriber
:Subscriber rdf:type owl:Class ;
            rdfs:subClassOf :Tool ;
            rdfs:comment "A subscriber requests information about a specific topic in a publish/subscribe network and receives messages from more publishers. A subscription is a request sent by the subscriber to receive messages on a particular topic."^^xsd:string ;
            rdfs:label "Subscriber"^^xsd:string .


###  https://w3id.org/iot-tta#Support
:Support rdf:type owl:Class ;
         rdfs:subClassOf :IoTLayers ;
         rdfs:comment "\"Support\" represents a layer of the IoT architecture. The support layer is represented by distributed systems (cloud systems)."^^xsd:string ;
         rdfs:label "Support"^^xsd:string .


###  https://w3id.org/iot-tta#Switch
:Switch rdf:type owl:Class ;
        rdfs:subClassOf :Computer_architecture ;
        rdfs:comment "In a computer network, a switch interconnects different network segments based on Media Access Control (MAC) addresses. A MAC address is a 6-byte integer on Token-ring or Ethernet networks used to identify a computer on a local network."^^xsd:string ;
        rdfs:label "Switch"^^xsd:string .


###  https://w3id.org/iot-tta#TCP
:TCP rdf:type owl:Class ;
     rdfs:subClassOf :Protocol ;
     rdfs:comment "TCP (Transmission Control Protocol) corresponds to the Transport layer of the Internet protocol suite TCP/IP. Common applications using TCP are the World Wide Web (WWW), e-mail, and file transfer (FTP)."^^xsd:string ;
     rdfs:label "TCP"^^xsd:string .


###  https://w3id.org/iot-tta#Technology
:Technology rdf:type owl:Class ;
            rdfs:subClassOf :Support ;
            rdfs:comment "Technologies used for distributed systems: Blockchain, big data processing, edge technology, computer cluster, data analysis, deep learning, etc."^^xsd:string ;
            rdfs:label "Technology"^^xsd:string .


###  https://w3id.org/iot-tta#Tool
:Tool rdf:type owl:Class ;
      rdfs:subClassOf :Support ;
      rdfs:comment "Tools for distributed computing technologies like MapReduce, Cloudera, Spark, HBase, Hortonworks, Subscriber, Watson IoT, etc."^^xsd:string ;
      rdfs:label "Tool"^^xsd:string .


###  https://w3id.org/iot-tta#Transducer
:Transducer rdf:type owl:Class ;
            rdfs:subClassOf :Sensor_Actuator ;
            rdfs:comment "A transducer converts a signal from one physical structure to another and converts one type of energy into another type. There are two types of transducers: sensors and actuators. Sensors are used for sensing things and devices etc."^^xsd:string ;
            rdfs:label "Transducer"^^xsd:string .


###  https://w3id.org/iot-tta#UDP
:UDP rdf:type owl:Class ;
     rdfs:subClassOf :Protocol ;
     rdfs:comment "UDP (User Datagram Protocol) corresponds to the Transport layer of the Internet protocol suite TCP/IP. UDP ensures the delivery of messages over a network, but unlike the TCP protocol, information packets are generally sent without receipt confirmation."^^xsd:string ;
     rdfs:label "UDP"^^xsd:string .


###  https://w3id.org/iot-tta#WPAN
:WPAN rdf:type owl:Class ;
      rdfs:subClassOf :Protocol ;
      rdfs:comment "WPAN (Wireless Personal Area Network) is a PAN that ensures the connection between devices through wireless, within a radius of 10 meters. WPAN includes wearable devices, USB flash drives, wireless mouse, Bluetooth, Wi-Fi, thermostats, security systems, lighting controls, motion sensors, etc."^^xsd:string ;
      rdfs:label "WPAN"^^xsd:string .


###  https://w3id.org/iot-tta#Watson_IoT
:Watson_IoT rdf:type owl:Class ;
            rdfs:subClassOf :Tool ;
            rdfs:comment "IBM Watson IoT Platform manages connected devices and offers access to live and historical data for IoT applications."^^xsd:string ;
            rdfs:label "Watson_IoT"^^xsd:string .


###  https://w3id.org/iot-tta#Web_Technology
:Web_Technology rdf:type owl:Class ;
                rdfs:subClassOf :Logic ;
                rdfs:comment "Hardware components of an IoT system are integrated with certain Web technologies and software platforms."^^xsd:string ;
                rdfs:label "Web_Technology"^^xsd:string .


###  https://w3id.org/iot-tta#Web_socket
:Web_socket rdf:type owl:Class ;
            rdfs:subClassOf :Application ;
            rdfs:comment "Applications that use the WebSocket API"^^xsd:string ;
            rdfs:label "Web_socket"^^xsd:string .


###  https://w3id.org/iot-tta#Wireless_sensor_network
:Wireless_sensor_network rdf:type owl:Class ;
                         rdfs:subClassOf :Sensor_Actuator ;
                         rdfs:comment "Wireless Sensor Networks - Sensor nodes are used with an onboard processor that manages and monitors the environment in a certain area. They are connected to the base station through the Internet to share data."^^xsd:string ;
                         rdfs:label "Wireless_sensor_network"^^xsd:string .


###  https://w3id.org/iot-tta#XML
:XML rdf:type owl:Class ;
     rdfs:subClassOf :Internet_standard ;
     rdfs:comment "XML (Extensible Markup Language) is a markup language recommended by the W3C (World Wide Web Consortium) and used for storing unstructured and semi-structured data and transferring data between Internet applications."^^xsd:string ;
     rdfs:label "XML"^^xsd:string .


###  https://w3id.org/iot-tta#XMPP
:XMPP rdf:type owl:Class ;
      rdfs:subClassOf :Protocol ;
      rdfs:comment "XMPP (Extensible Messaging and Presence Protocol) is an open standard that offers support for middleware applications, invisible messaging with the TCP network layer (hides the details of messaging), voice and video calls, collaboration, and generalized routing of XML data."^^xsd:string ;
      rdfs:label "XMPP"^^xsd:string .


###  https://w3id.org/iot-tta#YARN
:YARN rdf:type owl:Class ;
      rdfs:subClassOf :Distributed_operating_system ;
      rdfs:comment "Yarn (Yet Another Resource Negotiator) is a distributed operating system. YARN allows the resource management and scheduling jobs in Hadoop."^^xsd:string ;
      rdfs:label "YARN"^^xsd:string .


###  https://w3id.org/iot-tta#health-monitoring_system
:health-monitoring_system rdf:type owl:Class ;
                          rdfs:subClassOf :Smart_Product ;
                          rdfs:comment "Remote patient monitoring devices: glucometer, pulse oximeter, thermometer, ECG, digital stethoscope, wearables, scales, etc."^^xsd:string ;
                          rdfs:label "health-monitoring_system"^^xsd:string .


###  https://w3id.org/iot-tta#iBeacon
:iBeacon rdf:type owl:Class ;
         rdfs:subClassOf :Smart_Product ;
         rdfs:comment "iBeacon from Apple and Eddystone from Google are portable electronic devices that use network protocols such as NFC, RFID, optical tags, or BLE as hardware transmitters."^^xsd:string ;
         rdfs:label "iBeacon"^^xsd:string .


#################################################################
#    Individuals
#################################################################

###  https://w3id.org/iot-tta
<https://w3id.org/iot-tta> rdf:type owl:NamedIndividual ,
                                    voaf:Vocabulary .


###  https://w3id.org/iot-tta#Access_control
:Access_control rdf:type owl:NamedIndividual ,
                         :Blockchain_solution ;
                rdfs:comment "access_control (Individual): a Blockchain solution"^^xsd:string ;
                rdfs:label "access_control"^^xsd:string .


###  https://w3id.org/iot-tta#Apache_Hadoop
:Apache_Hadoop rdf:type owl:NamedIndividual ,
                        :Tool ;
               :isToolFor :Large_data_stream ;
               rdfs:comment "apache_Hadoop (Individual): a Tool with Object property assertions (isToolFor)"^^xsd:string ;
               rdfs:label "apache_Hadoop"^^xsd:string .


###  https://w3id.org/iot-tta#Apache_IoT_edge
:Apache_IoT_edge rdf:type owl:NamedIndividual ,
                          :Tool ;
                 rdfs:comment "apache_IoT_edge (Individual): a Tool"^^xsd:string ;
                 rdfs:label "apache_IoT_edge"^^xsd:string .


###  https://w3id.org/iot-tta#Autonomous_vehicle
:Autonomous_vehicle rdf:type owl:NamedIndividual ,
                             :Edge_application ;
                    :hasTechnology :Micro_data_center ;
                    rdfs:comment "autonomous_vehicle (Individual): an Edge application with Object property assertions (hasTechnology)"^^xsd:string ;
                    rdfs:label "autonomous_vehicle"^^xsd:string .


###  https://w3id.org/iot-tta#Avoid_synchronization
:Avoid_synchronization rdf:type owl:NamedIndividual ,
                                :Cloud_service ;
                       rdfs:comment "avoid_synchronization (Individual): a Cloud service"^^xsd:string ;
                       rdfs:label "avoid_synchronization"^^xsd:string .


###  https://w3id.org/iot-tta#Azure_IoT_edge
:Azure_IoT_edge rdf:type owl:NamedIndividual ,
                         :Tool ;
                rdfs:comment "azure_IoT_edge (Individual): a Tool"^^xsd:string ;
                rdfs:label "azure_IoT_edge"^^xsd:string .


###  https://w3id.org/iot-tta#BACnet
:BACnet rdf:type owl:NamedIndividual ,
                 :SCADA_common_protocol ;
        :Lack_security_measure :Threats_at_critical_infrastructure ;
        :Protocols_were_layered :Ethernet ;
        rdfs:comment "bacNet (Individual): a SCADA common protocol with Object property assertions (Protocols_were_layered, Lack_security_measure)"^^xsd:string ;
        rdfs:label "bacNet"^^xsd:string .


###  https://w3id.org/iot-tta#Blockchain_algorithm
:Blockchain_algorithm rdf:type owl:NamedIndividual ,
                               :Blockchain ;
                      :hasProblem :Energy_managed ;
                      rdfs:comment "blockchain_algorithm (Individual): of Blockchain type with Object property assertions (hasProblem)"^^xsd:string ;
                      rdfs:label "blockchain_algorithm"^^xsd:string .


###  https://w3id.org/iot-tta#Centralized_service
:Centralized_service rdf:type owl:NamedIndividual ,
                              :Cloud_service ;
                     rdfs:comment "centralized_service (Individual): a Cloud service"^^xsd:string ;
                     rdfs:label "centralized_service"^^xsd:string .


###  https://w3id.org/iot-tta#Cloud_Photon1
:Cloud_Photon1 rdf:type owl:NamedIndividual ,
                        :Particle_cloud ;
               :request :Thingspeak1 ;
               rdfs:comment "cloud_Photon1 (Individual): a Particle_cloud with Object property assertions (request)"^^xsd:string ;
               rdfs:label "cloud_Photon1"^^xsd:string .


###  https://w3id.org/iot-tta#Cloud_Photon2
:Cloud_Photon2 rdf:type owl:NamedIndividual ,
                        :Particle_cloud ;
               :request :Thingspeak2 ;
               rdfs:comment "cloud_Photon2 (Individual): a Particle_cloud with Object property assertions (request)"^^xsd:string ;
               rdfs:label "cloud_Photon2"^^xsd:string .


###  https://w3id.org/iot-tta#Cloud_gaming
:Cloud_gaming rdf:type owl:NamedIndividual ,
                       :Edge_application ;
              :hasTechnology :Micro_data_center ;
              rdfs:comment "cloud_gaming (Individual): an Edge application with Object property assertions (hasTechnology)"^^xsd:string ;
              rdfs:label "cloud_gaming"^^xsd:string .


###  https://w3id.org/iot-tta#Cluster1
:Cluster1 rdf:type owl:NamedIndividual ,
                   :Computer_cluster ;
          rdfs:comment "cluster1 (Individual): a Computer cluster"^^xsd:string ;
          rdfs:label "cluster1"^^xsd:string .


###  https://w3id.org/iot-tta#Cluster2
:Cluster2 rdf:type owl:NamedIndividual ,
                   :Computer_cluster ;
          rdfs:comment "cluster2 (Individual): a Computer cluster"^^xsd:string ;
          rdfs:label "cluster2"^^xsd:string .


###  https://w3id.org/iot-tta#Computational_cost
:Computational_cost rdf:type owl:NamedIndividual ,
                             :Edge_security ;
                    :best_Practices :Smart_grid ;
                    :has_SecuritySolution :Correct_Edge_implementation ;
                    rdfs:comment "computational_cost (Individual): of Edge security type with Object property assertions (has_SecuritySolution, best_Practices)"^^xsd:string ;
                    rdfs:label "computational_cost"^^xsd:string .


###  https://w3id.org/iot-tta#Connection1
:Connection1 rdf:type owl:NamedIndividual ,
                      :Flow ;
             :read :Particle_publish1 ;
             :hasValueConnection 1 ;
             rdfs:comment "connection1 (Individual): a Flow with Object property assertions (read), Data property assertions (hasValueConnection)"^^xsd:string ;
             rdfs:label "connection1"^^xsd:string .


###  https://w3id.org/iot-tta#Connection2
:Connection2 rdf:type owl:NamedIndividual ,
                      :Flow ;
             :read :Particle_publish2 ;
             :hasValueConnection 0 ;
             rdfs:comment "connection2 (Individual): a Flow with Object property assertions (read), Data property assertions (hasValueConnection)"^^xsd:string ;
             rdfs:label "connection2"^^xsd:string .


###  https://w3id.org/iot-tta#Correct_Edge_implementation
:Correct_Edge_implementation rdf:type owl:NamedIndividual ,
                                      :Blockchain_solution ;
                             rdfs:comment "correct_Edge_implementation (Individual): a Blockchain solution"^^xsd:string ;
                             rdfs:label "correct_Edge_implementation"^^xsd:string .


###  https://w3id.org/iot-tta#DC1
:DC1 rdf:type owl:NamedIndividual ,
              :Data_center ;
     :hasService :Centralized_service ;
     :useAlgorithm :Paxos ;
     rdfs:comment "dc1 (Individual): a Data center with Object property assertions (hasService, useAlgorithm)"^^xsd:string ;
     rdfs:label "dc1"^^xsd:string .


###  https://w3id.org/iot-tta#DC2
:DC2 rdf:type owl:NamedIndividual ,
              :Data_center ;
     :hasService :Avoid_synchronization ;
     :useAlgorithm :Zookeeper ;
     rdfs:comment "dc2 (Individual): a Data center with Object property assertions (hasService, useAlgorithm)"^^xsd:string ;
     rdfs:label "dc2"^^xsd:string .


###  https://w3id.org/iot-tta#DC3
:DC3 rdf:type owl:NamedIndividual ,
              :Data_center ;
     :hasService :Avoid_synchronization ;
     :useAlgorithm :Paxos ;
     rdfs:comment "dc3 (Individual): a Data center with Object property assertions (hasService, useAlgorithm)"^^xsd:string ;
     rdfs:label "dc3"^^xsd:string .


###  https://w3id.org/iot-tta#DC4
:DC4 rdf:type owl:NamedIndividual ,
              :Data_center ;
     :useAlgorithm :Paxos ;
     rdfs:comment "dc4 (Individual): a Data center with Object property assertions (useAlgorithm)"^^xsd:string ;
     rdfs:label "dc4"^^xsd:string .


###  https://w3id.org/iot-tta#Data_protection
:Data_protection rdf:type owl:NamedIndividual ,
                          :Blockchain_solution ;
                 rdfs:comment "data_protection (Individual): a Blockchain solution with Object property assertions (hasSolution)"^^xsd:string ;
                 rdfs:label "data_protection"^^xsd:string .


###  https://w3id.org/iot-tta#Data_security_risk
:Data_security_risk rdf:type owl:NamedIndividual ,
                             :SCADA_problem ;
                    :countermeasure :End-to-end_encryption ,
                                    :Strong_authentication ;
                    rdfs:comment "data_security_risk (Individual): a SCADA problem with Object property assertions (countermeasure)"^^xsd:string ;
                    rdfs:label "data_security_risk"^^xsd:string .


###  https://w3id.org/iot-tta#Data_stream_continue
:Data_stream_continue rdf:type owl:NamedIndividual ,
                               :Blockchain ;
                      :hasProblem :Throughput_limited ;
                      rdfs:comment "data_stream_continue (Individual): of Blockchain type with Object property assertions (hasProblem)"^^xsd:string ;
                      rdfs:label "data_stream_continue"^^xsd:string .


###  https://w3id.org/iot-tta#Deep_learning_algorithm
:Deep_learning_algorithm rdf:type owl:NamedIndividual ,
                                  :Deep_learning ;
                         :hasTool :Tensor_Flow ,
                                  :Theano ;
                         rdfs:comment "deep_learning_algorithm (Individual): of Deep learning type with Object property assertions (hasTool)"^^xsd:string ;
                         rdfs:label "deep_learning_algorithm"^^xsd:string .


###  https://w3id.org/iot-tta#Distributed_authentication
:Distributed_authentication rdf:type owl:NamedIndividual ,
                                     :Blockchain_solution ;
                            rdfs:comment "distributed_authentication (Individual): a Blockchain solution"^^xsd:string ;
                            rdfs:label "distributed_authentication"^^xsd:string .


###  https://w3id.org/iot-tta#Distributed_capability
:Distributed_capability rdf:type owl:NamedIndividual ,
                                 :BigData_capability ;
                        rdfs:comment "distributed_capability (Individual): Big data capability"^^xsd:string ;
                        rdfs:label "distributed_capability"^^xsd:string .


###  https://w3id.org/iot-tta#End-to-end_encryption
:End-to-end_encryption rdf:type owl:NamedIndividual ,
                                :SCADA_solution ;
                       rdfs:comment "end-to-end_encryption (Object property): a SCADA_solution"^^xsd:string ;
                       rdfs:label "end-to-end_encryption"^^xsd:string .


###  https://w3id.org/iot-tta#Energy_managed
:Energy_managed rdf:type owl:NamedIndividual ,
                         :Blockchain_problem ;
                :hasSolution :Improve_central_algorithm ;
                rdfs:comment "energy_managed (Individual): a Blockchain problem with Object property assertions (hasSolution)"^^xsd:string ;
                rdfs:label "energy_managed"^^xsd:string .


###  https://w3id.org/iot-tta#Ethernet
:Ethernet rdf:type owl:NamedIndividual ,
                   :SCADA_today_protocol ;
          :Support_communication :Long-distance_communication ;
          rdfs:comment "ethernet (Individual): a SCADA todat protocol with Object property assertions (Support_communication)"^^xsd:string ;
          rdfs:label "ethernet"^^xsd:string .


###  https://w3id.org/iot-tta#Hadoop
:Hadoop rdf:type owl:NamedIndividual ,
                 :Tool ;
        :isUsedBy :Cluster1 ,
                  :Cluster2 ;
        rdfs:comment "hadoop (Individual): a Tool with Object property assertions (isUsedBy)"^^xsd:string ;
        rdfs:label "hadoop"^^xsd:string .


###  https://w3id.org/iot-tta#Improve_central_algorithm
:Improve_central_algorithm rdf:type owl:NamedIndividual ,
                                    :Blockchain_solution ;
                           rdfs:comment "improve_central_algorithm (Individual): a Blockchain solution"^^xsd:string ;
                           rdfs:label "improve_central_algorithm"^^xsd:string .


###  https://w3id.org/iot-tta#Integrity_assurance
:Integrity_assurance rdf:type owl:NamedIndividual ,
                              :Blockchain_solution ;
                     rdfs:comment "integrity_assurance (Individual): a Blockchain solution"^^xsd:string ;
                     rdfs:label "integrity_assurance"^^xsd:string .


###  https://w3id.org/iot-tta#Large_data_stream
:Large_data_stream rdf:type owl:NamedIndividual ,
                            :BigData ;
                   :isProcessed :Distributed_capability ;
                   rdfs:comment "large_data_stream (Individual): Big Data type with Object property assertions (isProcessed)"^^xsd:string ;
                   rdfs:label "large_data_stream"^^xsd:string .


###  https://w3id.org/iot-tta#Long-distance_communication
:Long-distance_communication rdf:type owl:NamedIndividual ,
                                      :SCADA_capability ;
                             rdfs:comment "long-distance_communication (Individual): a SCADA_capability"^^xsd:string ;
                             rdfs:label "long-distance_communication"^^xsd:string .


###  https://w3id.org/iot-tta#Maintain_configuration
:Maintain_configuration rdf:type owl:NamedIndividual ,
                                 :Cloud_service ;
                        rdfs:comment "maintain_configuration (Individual): a Cloud service"^^xsd:string ;
                        rdfs:label "maintain_configuration"^^xsd:string .


###  https://w3id.org/iot-tta#MapReduce
:MapReduce rdf:type owl:NamedIndividual ,
                    :Tool ;
           :isApplied :Cluster1 ;
           rdfs:comment "mapReduce (Individual): a Tool with Object property assertions (isApplied)"^^xsd:string ;
           rdfs:label "mapReduce"^^xsd:string .


###  https://w3id.org/iot-tta#Micro_data_center
:Micro_data_center rdf:type owl:NamedIndividual ,
                            :Edge_technology ;
                   :hasTool :Azure_IoT_edge ;
                   rdfs:comment "micro_data_center (Individual): an edge technology with Object property assertions (hasTool)"^^xsd:string ;
                   rdfs:label "micro_data_center"^^xsd:string .


###  https://w3id.org/iot-tta#Modbus
:Modbus rdf:type owl:NamedIndividual ,
                 :SCADA_common_protocol ;
        :Lack_security_measure :Threats_at_critical_infrastructure ;
        :Protocols_were_layered :TCP_IP ;
        rdfs:comment "modbus (Individual): a SCADA common protocol with Object property assertions (Lack_security_measure, Protocols_were_layered)"^^xsd:string ;
        rdfs:label "modbus"^^xsd:string .


###  https://w3id.org/iot-tta#OPC_servers
:OPC_servers rdf:type owl:NamedIndividual ,
                      :Edge_technology ;
             :hasTool :Apache_IoT_edge ;
             rdfs:comment "opc_servers (Individual): an edge technology with Object property assertions (hasTool)"^^xsd:string ;
             rdfs:label "opc_servers"^^xsd:string .


###  https://w3id.org/iot-tta#Oven1
:Oven1 rdf:type owl:NamedIndividual ,
                :Industrial_oven ;
       :hasTemperatureRange "508.0"^^xsd:double ;
       rdfs:comment "oven1 (Individual): an Industrial_oven with Data property assertions (hasTemperatureRange)"^^xsd:string ;
       rdfs:label "oven1"^^xsd:string .


###  https://w3id.org/iot-tta#Oven2
:Oven2 rdf:type owl:NamedIndividual ,
                :Industrial_oven ;
       :hasTemperatureRange "502.0"^^xsd:double ;
       rdfs:comment "oven2 (Individual): an Industrial_oven with Data property assertions (hasTemperatureRange)"^^xsd:string ;
       rdfs:label "oven2"^^xsd:string .


###  https://w3id.org/iot-tta#Oven3
:Oven3 rdf:type owl:NamedIndividual ,
                :Industrial_oven ;
       :hasTemperatureRange "501.0"^^xsd:double ;
       rdfs:comment "oven3 (Individual): an Industrial_oven with Data property assertions (hasTemperatureRange)"^^xsd:string ;
       rdfs:label "oven3"^^xsd:string .


###  https://w3id.org/iot-tta#Oven4
:Oven4 rdf:type owl:NamedIndividual ,
                :Industrial_oven ;
       :hasTemperatureRange "506.0"^^xsd:double ;
       rdfs:comment "oven4 (Individual): an Industrial_oven with Data property assertions (hasTemperatureRange)"^^xsd:string ;
       rdfs:label "oven4"^^xsd:string .


###  https://w3id.org/iot-tta#Oven5
:Oven5 rdf:type owl:NamedIndividual ,
                :Industrial_oven ;
       rdfs:comment "oven5 (Individual): an Industrial_oven"^^xsd:string ;
       rdfs:label "oven5"^^xsd:string .


###  https://w3id.org/iot-tta#Particle_publish1
:Particle_publish1 rdf:type owl:NamedIndividual ,
                            :Firmware ;
                   :send :Cloud_Photon1 ;
                   :hasTimeLimit 30 ;
                   rdfs:comment "particle_publish1 (Individual): a Firmware with Object property assertions (send), Data property assertions (hasTimeLimit)"^^xsd:string ;
                   rdfs:label "particle_publish1"^^xsd:string .


###  https://w3id.org/iot-tta#Particle_publish2
:Particle_publish2 rdf:type owl:NamedIndividual ,
                            :Firmware ;
                   :send :Cloud_Photon2 ;
                   :hasTimeLimit 25 ;
                   rdfs:comment "particle_publish2 (Individual): a Firmware with Object property assertions (send), Data property assertions (hasTimeLimit)"^^xsd:string ;
                   rdfs:label "particle_publish2"^^xsd:string .


###  https://w3id.org/iot-tta#Paxos
:Paxos rdf:type owl:NamedIndividual ,
                :Data_center ;
       :isApplied :DC1 ,
                  :DC3 ,
                  :DC4 ;
       rdfs:comment "paxos (Individual): a Data center with Object property assertions (isApplied)"^^xsd:string ;
       rdfs:label "paxos"^^xsd:string .


###  https://w3id.org/iot-tta#Photon1
:Photon1 rdf:type owl:NamedIndividual ,
                  :Particle_Photon ;
         :wire :Connection1 ;
         rdfs:comment "photon1 (Individual): a Particle_Photon with Object property assertions (wire)"^^xsd:string ;
         rdfs:label "photon1"^^xsd:string .


###  https://w3id.org/iot-tta#Photon2
:Photon2 rdf:type owl:NamedIndividual ,
                  :Particle_Photon ;
         :wire :Connection2 ;
         rdfs:comment "photon2 (Individual): a Particle_Photon with Object property assertions (wire)"^^xsd:string ;
         rdfs:label "photon2"^^xsd:string .


###  https://w3id.org/iot-tta#Predictive_maintenance
:Predictive_maintenance rdf:type owl:NamedIndividual ,
                                 :Edge_application ;
                        :hasTechnology :OPC_servers ;
                        rdfs:comment "predictive_maintenance (Individual): an Edge application with Object property assertions (hasTechnology)"^^xsd:string ;
                        rdfs:label "predictive_maintenance"^^xsd:string .


###  https://w3id.org/iot-tta#RTD3
:RTD3 rdf:type owl:NamedIndividual ,
               :RTD_sensor ;
      :heat :Oven3 ;
      :hasAccuracy "0.6"^^xsd:float ;
      :provideHeat "510.0"^^xsd:double ;
      rdfs:comment "rtdSensor3 (Individual): an RTD_sensor with Object property assertions (heat), Data property assertions (provideHeat, hasAccuracy)"^^xsd:string ;
      rdfs:label "rtdSensor3"^^xsd:string .


###  https://w3id.org/iot-tta#RTD4
:RTD4 rdf:type owl:NamedIndividual ,
               :RTD_sensor ;
      :heat :Oven4 ;
      :hasAccuracy "0.8"^^xsd:float ;
      :provideHeat "520.0"^^xsd:double ;
      rdfs:comment "rtdSensor4 (Individual): an RTD_sensor with Object property assertions (heat), Data property assertions (provideHeat, hasAccuracy)"^^xsd:string ;
      rdfs:label "rtdSensor4"^^xsd:string .


###  https://w3id.org/iot-tta#RTD5
:RTD5 rdf:type owl:NamedIndividual ,
               :RTD_sensor ;
      :heat :Oven5 ;
      rdfs:comment "rtdSensor5 (Individual): an RTD_sensor with Object property assertions (heat)"^^xsd:string ;
      rdfs:label "rtdSensor5"^^xsd:string .


###  https://w3id.org/iot-tta#RTDsensor1
:RTDsensor1 rdf:type owl:NamedIndividual ,
                     :RTD_sensor ;
            :heat :Oven1 ;
            :hasAccuracy "0.5"^^xsd:float ;
            :provideHeat "480.0"^^xsd:double ;
            rdfs:comment "rtdSensor1 (Individual): an RTD_sensor with Object property assertions (heat), Data property assertions (provideHeat, hasAccuracy)"^^xsd:string ;
            rdfs:label "rtdSensor1"^^xsd:string .


###  https://w3id.org/iot-tta#RTDsensor2
:RTDsensor2 rdf:type owl:NamedIndividual ,
                     :RTD_sensor ;
            :heat :Oven2 ;
            :hasAccuracy "0.3"^^xsd:float ;
            :provideHeat "500.0"^^xsd:double ;
            rdfs:comment "rtdSensor2 (Individual): an RTD_sensor with Object property assertions (heat), Data property assertions (provideHeat, hasAccuracy)"^^xsd:string ;
            rdfs:label "rtdSensor2"^^xsd:string .


###  https://w3id.org/iot-tta#Reducing_latency_in_sending_data
:Reducing_latency_in_sending_data rdf:type owl:NamedIndividual ,
                                           :Blockchain_solution ;
                                  rdfs:comment "reducing_latency_in_sending_data (Individual): a Blockchain solution"^^xsd:string ;
                                  rdfs:label "reducing_latency_in_sending_data"^^xsd:string .


###  https://w3id.org/iot-tta#SCADA_application
:SCADA_application rdf:type owl:NamedIndividual ,
                            :SCADA ;
                   :threats_to_data_security :Data_security_risk ;
                   rdfs:comment "scada_application (Individual): of SCADA type with Object property assertions (threats_to_data_security)"^^xsd:string ;
                   rdfs:label "scada_application"^^xsd:string .


###  https://w3id.org/iot-tta#SCADA_system
:SCADA_system rdf:type owl:NamedIndividual ,
                       :SCADA ;
              rdfs:comment "scada_system (Individual): SCADA type"^^xsd:string ;
              rdfs:label "scada_system"^^xsd:string .


###  https://w3id.org/iot-tta#Secure_key_management
:Secure_key_management rdf:type owl:NamedIndividual ,
                                :Blockchain_solution ;
                       rdfs:comment "secure_key_management (Individual): a Blockchain solution"^^xsd:string ;
                       rdfs:label "secure_key_management"^^xsd:string .


###  https://w3id.org/iot-tta#Security_problem
:Security_problem rdf:type owl:NamedIndividual ,
                           :Blockchain_security ;
                  :hasSolution :Access_control ,
                               :Data_protection ,
                               :Integrity_assurance ,
                               :Secure_key_management ;
                  rdfs:comment "security_problem (Individual): a Blockchain security type with Object property assertions (hasSolution)"^^xsd:string ;
                  rdfs:label "security_problem"^^xsd:string .


###  https://w3id.org/iot-tta#Smart_contracts
:Smart_contracts rdf:type owl:NamedIndividual ,
                          :Blockchain ;
                 :hasSecurity_problem :Security_problem ;
                 rdfs:comment "smart_contracts (Individual): of Blockchain type with Object property assertions (hasSecurity)"^^xsd:string ;
                 rdfs:label "smart_contracts"^^xsd:string .


###  https://w3id.org/iot-tta#Smart_grid
:Smart_grid rdf:type owl:NamedIndividual ,
                     :Edge_application ;
            :hasTechnology :OPC_servers ;
            rdfs:comment "smart_grid (Individual): an Edge application with Object property assertions (hasTechnology)"^^xsd:string ;
            rdfs:label "smart_grid"^^xsd:string .


###  https://w3id.org/iot-tta#Smart_home
:Smart_home rdf:type owl:NamedIndividual ,
                     :Edge_application ;
            :hasTechnology :OPC_servers ;
            rdfs:comment "smart_home (Individual): an Edge application with Object property assertions (hasTechnology)"^^xsd:string ;
            rdfs:label "smart_home"^^xsd:string .


###  https://w3id.org/iot-tta#Strong_authentication
:Strong_authentication rdf:type owl:NamedIndividual ,
                                :SCADA_solution ;
                       rdfs:comment "strong_authentication (Object property): a SCADA_solution"^^xsd:string ;
                       rdfs:label "strong_authentication"^^xsd:string .


###  https://w3id.org/iot-tta#Synchronization_in_throughput
:Synchronization_in_throughput rdf:type owl:NamedIndividual ,
                                        :Blockchain_solution ;
                               rdfs:comment "synchronization_in_throughput (Individual): a Blockchain solution"^^xsd:string ;
                               rdfs:label "synchronization_in_throughput"^^xsd:string .


###  https://w3id.org/iot-tta#TCP_IP
:TCP_IP rdf:type owl:NamedIndividual ,
                 :SCADA_today_protocol ;
        :Support_communication :Long-distance_communication ;
        rdfs:comment "tcp_IP (Individual): a SCADA today protocol with Object property assertions (Support_communication)"^^xsd:string ;
        rdfs:label "tcp_IP"^^xsd:string .


###  https://w3id.org/iot-tta#Tensor_Flow
:Tensor_Flow rdf:type owl:NamedIndividual ,
                      :Tool ;
             :isToolFor :Deep_learning_algorithm ;
             rdfs:comment "tensor_Flow (Individual): a Tool with Object property assertions (isToolFor)"^^xsd:string ;
             rdfs:label "tensor_Flow"^^xsd:string .


###  https://w3id.org/iot-tta#Theano
:Theano rdf:type owl:NamedIndividual ,
                 :Tool ;
        :isToolFor :Deep_learning_algorithm ;
        rdfs:comment "theano (Individual): a Tool with Object property assertions (isToolFor)"^^xsd:string ;
        rdfs:label "theano"^^xsd:string .


###  https://w3id.org/iot-tta#Thingspeak1
:Thingspeak1 rdf:type owl:NamedIndividual ,
                      :Subscriber ;
             rdfs:comment "thingspeak1 (Individual): a Subscriber"^^xsd:string ;
             rdfs:label "thingspeak1"^^xsd:string .


###  https://w3id.org/iot-tta#Thingspeak2
:Thingspeak2 rdf:type owl:NamedIndividual ,
                      :Subscriber ;
             rdfs:comment "thingspeak2 (Individual): a Subscriber"^^xsd:string ;
             rdfs:label "thingspeak2"^^xsd:string .


###  https://w3id.org/iot-tta#Threats_at_critical_infrastructure
:Threats_at_critical_infrastructure rdf:type owl:NamedIndividual ,
                                             :SCADA_problem ;
                                    rdfs:comment "threats_at_critical_infrastructure (Individual): a SCADA problem"^^xsd:string ;
                                    rdfs:label "threats_at_critical_infrastructure"^^xsd:string .


###  https://w3id.org/iot-tta#Throughput_limited
:Throughput_limited rdf:type owl:NamedIndividual ,
                             :Blockchain_problem ;
                    :hasSolution :Synchronization_in_throughput ;
                    rdfs:comment "throughput_limited (Individual): a Blockchain problem with Object property assertions (hasSolution)"^^xsd:string ;
                    rdfs:label "throughput_limited"^^xsd:string .


###  https://w3id.org/iot-tta#Transmission_speed
:Transmission_speed rdf:type owl:NamedIndividual ,
                             :Edge_security ;
                    :best_Practices :Smart_home ;
                    :has_SecuritySolution :Reducing_latency_in_sending_data ;
                    rdfs:comment "transmission_speed (Individual): of Edge security type with Object property assertions (has_SecuritySolution, best_Practices)"^^xsd:string ;
                    rdfs:label "transmission_speed"^^xsd:string .


###  https://w3id.org/iot-tta#Zookeeper
:Zookeeper rdf:type owl:NamedIndividual ,
                    :Data_center ;
           :hasService :Maintain_configuration ;
           :isApplied :DC2 ;
           rdfs:comment "zookeeper (Individual): a Data center with Object property assertions (isApplied, hasService)"^^xsd:string ;
           rdfs:label "zookeeper"^^xsd:string .


#################################################################
#    Annotations
#################################################################

owl:Thing rdfs:comment "IoT-TTA is a semantic ontology for Internet of Things technologies, tools, and applications."^^xsd:string ;
          rdfs:seeAlso ""^^xsd:string .


#################################################################
#    General axioms
#################################################################

[ rdf:type owl:AllDisjointClasses ;
  owl:members ( :Algorithm
                :Programming_Language
                :Web_Technology
              )
] .


[ rdf:type owl:AllDisjointClasses ;
  owl:members ( :Arduino
                :Particle_Photon
                :Raspberry_Pi
              )
] .


[ rdf:type owl:AllDisjointClasses ;
  owl:members ( :BLE
                :HTTP
                :IP
                :LoWPAN
                :MQTT
                :NFC_tag
                :Optical_tag
                :PAN
                :RFID_tag
                :SAMPL
                :TCP
                :UDP
                :WPAN
                :XMPP
              )
] .


[ rdf:type owl:AllDisjointClasses ;
  owl:members ( :BigData_app
                :Machine_learning
                :SOA
                :Web_socket
              )
] .


[ rdf:type owl:AllDisjointClasses ;
  owl:members ( :C
                :Java
                :Python
              )
] .


[ rdf:type owl:AllDisjointClasses ;
  owl:members ( :Computer_architecture
                :Control_engineering
                :Data_transmission
              )
] .


[ rdf:type owl:AllDisjointClasses ;
  owl:members ( :Control_System
                :Electrical_Grids
                :Factory_Equipment
                :Factory_Floor
                :Gas_Meter
                :Oil_Pipeline_Control
              )
] .


[ rdf:type owl:AllDisjointClasses ;
  owl:members ( :Digital
                :Gateway
                :Sensor_Actuator
              )
] .


[ rdf:type owl:AllDisjointClasses ;
  owl:members ( :Ethics
                :Management
                :Privacy
                :Security
              )
] .


[ rdf:type owl:AllDisjointClasses ;
  owl:members ( :Hardware_Platform
                :Logic
                :Purpose-built_Device
                :Smart_Product
              )
] .


[ rdf:type owl:AllDisjointClasses ;
  owl:members ( :Mahout
                :Mllib
                :Spark
              )
] .


[ rdf:type owl:AllDifferent ;
  owl:distinctMembers ( :Particle_publish1
                        :Particle_publish2
                      )
] .


[ rdf:type owl:AllDifferent ;
  owl:distinctMembers ( :Thingspeak1
                        :Thingspeak2
                      )
] .


#################################################################
#    Rules
#################################################################

<http://w3id.org/iot-tta#x> rdf:type swrl:Variable .

<http://w3id.org/iot-tta#y> rdf:type swrl:Variable .

<http://w3id.org/iot-tta#z> rdf:type swrl:Variable .

:x rdf:type swrl:Variable .

:y rdf:type swrl:Variable .

:z rdf:type swrl:Variable .

<http://w3id.org/iot-tta/#x> rdf:type swrl:Variable .

<http://w3id.org/iot-tta/#z> rdf:type swrl:Variable .

<http://w3id.org/iot-tta/#y> rdf:type swrl:Variable .

<http://w3id.org/iot-tta#w> rdf:type swrl:Variable .

<http://w3id.org/iot-tta#q> rdf:type swrl:Variable .

<http://w3id.org/iot-tta#t> rdf:type swrl:Variable .

<http://w3id.org/iot-tta#s> rdf:type swrl:Variable .

[ swrla:isRuleEnabled "true"^^xsd:boolean ;
   rdfs:comment ""^^xsd:string ;
   rdfs:label "R9a-a"^^xsd:string ;
   rdf:type swrl:Imp ;
   swrl:body [ rdf:type swrl:AtomList ;
               rdf:first [ rdf:type swrl:IndividualPropertyAtom ;
                           swrl:propertyPredicate :hasTechnology ;
                           swrl:argument1 <http://w3id.org/iot-tta#x> ;
                           swrl:argument2 <http://w3id.org/iot-tta#y>
                         ] ;
               rdf:rest [ rdf:type swrl:AtomList ;
                          rdf:first [ rdf:type swrl:ClassAtom ;
                                      swrl:classPredicate :Edge_technology ;
                                      swrl:argument1 <http://w3id.org/iot-tta#y>
                                    ] ;
                          rdf:rest [ rdf:type swrl:AtomList ;
                                     rdf:first [ rdf:type swrl:ClassAtom ;
                                                 swrl:classPredicate :Application ;
                                                 swrl:argument1 <http://w3id.org/iot-tta#x>
                                               ] ;
                                     rdf:rest [ rdf:type swrl:AtomList ;
                                                rdf:first [ rdf:type swrl:IndividualPropertyAtom ;
                                                            swrl:propertyPredicate :hasTool ;
                                                            swrl:argument1 <http://w3id.org/iot-tta#y> ;
                                                            swrl:argument2 <http://w3id.org/iot-tta#z>
                                                          ] ;
                                                rdf:rest rdf:nil
                                              ]
                                   ]
                        ]
             ] ;
   swrl:head [ rdf:type swrl:AtomList ;
               rdf:first [ rdf:type swrl:IndividualPropertyAtom ;
                           swrl:propertyPredicate :supporting_tool ;
                           swrl:argument1 <http://w3id.org/iot-tta#x> ;
                           swrl:argument2 <http://w3id.org/iot-tta#z>
                         ] ;
               rdf:rest rdf:nil
             ]
 ] .

[ swrla:isRuleEnabled "true"^^xsd:boolean ;
   rdfs:comment ""^^xsd:string ;
   rdfs:label "R9a-b"^^xsd:string ;
   rdf:type swrl:Imp ;
   swrl:body [ rdf:type swrl:AtomList ;
               rdf:first [ rdf:type swrl:IndividualPropertyAtom ;
                           swrl:propertyPredicate :hasTechnology ;
                           swrl:argument1 <http://w3id.org/iot-tta#x> ;
                           swrl:argument2 <http://w3id.org/iot-tta#y>
                         ] ;
               rdf:rest [ rdf:type swrl:AtomList ;
                          rdf:first [ rdf:type swrl:ClassAtom ;
                                      swrl:classPredicate :Edge_technology ;
                                      swrl:argument1 <http://w3id.org/iot-tta#y>
                                    ] ;
                          rdf:rest [ rdf:type swrl:AtomList ;
                                     rdf:first [ rdf:type swrl:ClassAtom ;
                                                 swrl:classPredicate :Application ;
                                                 swrl:argument1 <http://w3id.org/iot-tta#x>
                                               ] ;
                                     rdf:rest [ rdf:type swrl:AtomList ;
                                                rdf:first [ rdf:type swrl:IndividualPropertyAtom ;
                                                            swrl:propertyPredicate :hasTool ;
                                                            swrl:argument1 <http://w3id.org/iot-tta#y> ;
                                                            swrl:argument2 <http://w3id.org/iot-tta#z>
                                                          ] ;
                                                rdf:rest rdf:nil
                                              ]
                                   ]
                        ]
             ] ;
   swrl:head [ rdf:type swrl:AtomList ;
               rdf:first [ rdf:type swrl:BuiltinAtom ;
                           swrl:builtin <http://sqwrl.stanford.edu/ontologies/built-ins/3.4/sqwrl.owl#select> ;
                           swrl:arguments ( <http://w3id.org/iot-tta#x>
                                            <http://w3id.org/iot-tta#y>
                                            <http://w3id.org/iot-tta#z>
                                          )
                         ] ;
               rdf:rest rdf:nil
             ]
 ] .

[ swrla:isRuleEnabled "true"^^xsd:boolean ;
   rdfs:comment ""^^xsd:string ;
   rdfs:label "R4s-a"^^xsd:string ;
   rdf:type swrl:Imp ;
   swrl:body [ rdf:type swrl:AtomList ;
               rdf:first [ rdf:type swrl:IndividualPropertyAtom ;
                           swrl:propertyPredicate :isToolFor ;
                           swrl:argument1 <http://w3id.org/iot-tta#x> ;
                           swrl:argument2 <http://w3id.org/iot-tta#y>
                         ] ;
               rdf:rest [ rdf:type swrl:AtomList ;
                          rdf:first [ rdf:type swrl:ClassAtom ;
                                      swrl:classPredicate :BigData_capability ;
                                      swrl:argument1 <http://w3id.org/iot-tta#z>
                                    ] ;
                          rdf:rest [ rdf:type swrl:AtomList ;
                                     rdf:first [ rdf:type swrl:IndividualPropertyAtom ;
                                                 swrl:propertyPredicate :isProcessed ;
                                                 swrl:argument1 <http://w3id.org/iot-tta#y> ;
                                                 swrl:argument2 <http://w3id.org/iot-tta#z>
                                               ] ;
                                     rdf:rest [ rdf:type swrl:AtomList ;
                                                rdf:first [ rdf:type swrl:ClassAtom ;
                                                            swrl:classPredicate :Tool ;
                                                            swrl:argument1 :Apache_Hadoop
                                                          ] ;
                                                rdf:rest rdf:nil
                                              ]
                                   ]
                        ]
             ] ;
   swrl:head [ rdf:type swrl:AtomList ;
               rdf:first [ rdf:type swrl:IndividualPropertyAtom ;
                           swrl:propertyPredicate :hasCapability ;
                           swrl:argument1 <http://w3id.org/iot-tta#x> ;
                           swrl:argument2 <http://w3id.org/iot-tta#z>
                         ] ;
               rdf:rest rdf:nil
             ]
 ] .

[ swrla:isRuleEnabled "true"^^xsd:boolean ;
   rdfs:comment ""^^xsd:string ;
   rdfs:label "R4s-b"^^xsd:string ;
   rdf:type swrl:Imp ;
   swrl:body [ rdf:type swrl:AtomList ;
               rdf:first [ rdf:type swrl:ClassAtom ;
                           swrl:classPredicate :BigData_capability ;
                           swrl:argument1 <http://w3id.org/iot-tta#z>
                         ] ;
               rdf:rest [ rdf:type swrl:AtomList ;
                          rdf:first [ rdf:type swrl:IndividualPropertyAtom ;
                                      swrl:propertyPredicate :isProcessed ;
                                      swrl:argument1 <http://w3id.org/iot-tta#y> ;
                                      swrl:argument2 <http://w3id.org/iot-tta#z>
                                    ] ;
                          rdf:rest [ rdf:type swrl:AtomList ;
                                     rdf:first [ rdf:type swrl:IndividualPropertyAtom ;
                                                 swrl:propertyPredicate :isToolFor ;
                                                 swrl:argument1 :Apache_Hadoop ;
                                                 swrl:argument2 <http://w3id.org/iot-tta#y>
                                               ] ;
                                     rdf:rest rdf:nil
                                   ]
                        ]
             ] ;
   swrl:head [ rdf:type swrl:AtomList ;
               rdf:first [ rdf:type swrl:BuiltinAtom ;
                           swrl:builtin <http://sqwrl.stanford.edu/ontologies/built-ins/3.4/sqwrl.owl#select> ;
                           swrl:arguments ( <http://w3id.org/iot-tta#y>
                                            <http://w3id.org/iot-tta#z>
                                          )
                         ] ;
               rdf:rest rdf:nil
             ]
 ] .

[ swrla:isRuleEnabled "true"^^xsd:boolean ;
   rdfs:comment ""^^xsd:string ;
   rdfs:label "R5a-a"^^xsd:string ;
   rdf:type swrl:Imp ;
   swrl:body [ rdf:type swrl:AtomList ;
               rdf:first [ rdf:type swrl:ClassAtom ;
                           swrl:classPredicate :Blockchain ;
                           swrl:argument1 <http://w3id.org/iot-tta#x>
                         ] ;
               rdf:rest [ rdf:type swrl:AtomList ;
                          rdf:first [ rdf:type swrl:ClassAtom ;
                                      swrl:classPredicate :Blockchain_problem ;
                                      swrl:argument1 <http://w3id.org/iot-tta#y>
                                    ] ;
                          rdf:rest [ rdf:type swrl:AtomList ;
                                     rdf:first [ rdf:type swrl:IndividualPropertyAtom ;
                                                 swrl:propertyPredicate :hasSolution ;
                                                 swrl:argument1 <http://w3id.org/iot-tta#y> ;
                                                 swrl:argument2 <http://w3id.org/iot-tta#z>
                                               ] ;
                                     rdf:rest [ rdf:type swrl:AtomList ;
                                                rdf:first [ rdf:type swrl:IndividualPropertyAtom ;
                                                            swrl:propertyPredicate :hasProblem ;
                                                            swrl:argument1 <http://w3id.org/iot-tta#x> ;
                                                            swrl:argument2 <http://w3id.org/iot-tta#y>
                                                          ] ;
                                                rdf:rest rdf:nil
                                              ]
                                   ]
                        ]
             ] ;
   swrl:head [ rdf:type swrl:AtomList ;
               rdf:first [ rdf:type swrl:IndividualPropertyAtom ;
                           swrl:propertyPredicate :challenge ;
                           swrl:argument1 <http://w3id.org/iot-tta#x> ;
                           swrl:argument2 <http://w3id.org/iot-tta#z>
                         ] ;
               rdf:rest rdf:nil
             ]
 ] .

[ swrla:isRuleEnabled "true"^^xsd:boolean ;
   rdfs:comment ""^^xsd:string ;
   rdfs:label "R5a-b"^^xsd:string ;
   rdf:type swrl:Imp ;
   swrl:body [ rdf:type swrl:AtomList ;
               rdf:first [ rdf:type swrl:ClassAtom ;
                           swrl:classPredicate :Blockchain ;
                           swrl:argument1 <http://w3id.org/iot-tta#x>
                         ] ;
               rdf:rest [ rdf:type swrl:AtomList ;
                          rdf:first [ rdf:type swrl:ClassAtom ;
                                      swrl:classPredicate :Blockchain_problem ;
                                      swrl:argument1 <http://w3id.org/iot-tta#y>
                                    ] ;
                          rdf:rest [ rdf:type swrl:AtomList ;
                                     rdf:first [ rdf:type swrl:IndividualPropertyAtom ;
                                                 swrl:propertyPredicate :hasSolution ;
                                                 swrl:argument1 <http://w3id.org/iot-tta#y> ;
                                                 swrl:argument2 <http://w3id.org/iot-tta#z>
                                               ] ;
                                     rdf:rest [ rdf:type swrl:AtomList ;
                                                rdf:first [ rdf:type swrl:IndividualPropertyAtom ;
                                                            swrl:propertyPredicate :hasProblem ;
                                                            swrl:argument1 <http://w3id.org/iot-tta#x> ;
                                                            swrl:argument2 <http://w3id.org/iot-tta#y>
                                                          ] ;
                                                rdf:rest rdf:nil
                                              ]
                                   ]
                        ]
             ] ;
   swrl:head [ rdf:type swrl:AtomList ;
               rdf:first [ rdf:type swrl:BuiltinAtom ;
                           swrl:builtin <http://sqwrl.stanford.edu/ontologies/built-ins/3.4/sqwrl.owl#select> ;
                           swrl:arguments ( <http://w3id.org/iot-tta#x>
                                            <http://w3id.org/iot-tta#y>
                                            <http://w3id.org/iot-tta#z>
                                          )
                         ] ;
               rdf:rest rdf:nil
             ]
 ] .

[ swrla:isRuleEnabled "true"^^xsd:boolean ;
   rdfs:comment ""^^xsd:string ;
   rdfs:label "R6a-b"^^xsd:string ;
   rdf:type swrl:Imp ;
   swrl:body [ rdf:type swrl:AtomList ;
               rdf:first [ rdf:type swrl:ClassAtom ;
                           swrl:classPredicate :Blockchain ;
                           swrl:argument1 <http://w3id.org/iot-tta#x>
                         ] ;
               rdf:rest [ rdf:type swrl:AtomList ;
                          rdf:first [ rdf:type swrl:ClassAtom ;
                                      swrl:classPredicate :Blockchain_security ;
                                      swrl:argument1 <http://w3id.org/iot-tta#y>
                                    ] ;
                          rdf:rest [ rdf:type swrl:AtomList ;
                                     rdf:first [ rdf:type swrl:IndividualPropertyAtom ;
                                                 swrl:propertyPredicate :hasSolution ;
                                                 swrl:argument1 <http://w3id.org/iot-tta#y> ;
                                                 swrl:argument2 <http://w3id.org/iot-tta#z>
                                               ] ;
                                     rdf:rest [ rdf:type swrl:AtomList ;
                                                rdf:first [ rdf:type swrl:IndividualPropertyAtom ;
                                                            swrl:propertyPredicate :hasSecurity_problem ;
                                                            swrl:argument1 <http://w3id.org/iot-tta#x> ;
                                                            swrl:argument2 <http://w3id.org/iot-tta#y>
                                                          ] ;
                                                rdf:rest rdf:nil
                                              ]
                                   ]
                        ]
             ] ;
   swrl:head [ rdf:type swrl:AtomList ;
               rdf:first [ rdf:type swrl:BuiltinAtom ;
                           swrl:builtin <http://sqwrl.stanford.edu/ontologies/built-ins/3.4/sqwrl.owl#select> ;
                           swrl:arguments ( <http://w3id.org/iot-tta#x>
                                            <http://w3id.org/iot-tta#y>
                                            <http://w3id.org/iot-tta#z>
                                          )
                         ] ;
               rdf:rest rdf:nil
             ]
 ] .

[ swrla:isRuleEnabled "true"^^xsd:boolean ;
   rdfs:comment ""^^xsd:string ;
   rdfs:label "R6a-a"^^xsd:string ;
   rdf:type swrl:Imp ;
   swrl:body [ rdf:type swrl:AtomList ;
               rdf:first [ rdf:type swrl:IndividualPropertyAtom ;
                           swrl:propertyPredicate :hasSecurity_problem ;
                           swrl:argument1 :Smart_contracts ;
                           swrl:argument2 <http://w3id.org/iot-tta#y>
                         ] ;
               rdf:rest [ rdf:type swrl:AtomList ;
                          rdf:first [ rdf:type swrl:ClassAtom ;
                                      swrl:classPredicate :Blockchain ;
                                      swrl:argument1 <http://w3id.org/iot-tta#x>
                                    ] ;
                          rdf:rest [ rdf:type swrl:AtomList ;
                                     rdf:first [ rdf:type swrl:IndividualPropertyAtom ;
                                                 swrl:propertyPredicate :hasSolution ;
                                                 swrl:argument1 <http://w3id.org/iot-tta#y> ;
                                                 swrl:argument2 <http://w3id.org/iot-tta#z>
                                               ] ;
                                     rdf:rest rdf:nil
                                   ]
                        ]
             ] ;
   swrl:head [ rdf:type swrl:AtomList ;
               rdf:first [ rdf:type swrl:IndividualPropertyAtom ;
                           swrl:propertyPredicate :challenge ;
                           swrl:argument1 <http://w3id.org/iot-tta#x> ;
                           swrl:argument2 <http://w3id.org/iot-tta#z>
                         ] ;
               rdf:rest rdf:nil
             ]
 ] .

[ swrla:isRuleEnabled "true"^^xsd:boolean ;
   rdfs:comment ""^^xsd:string ;
   rdfs:label "R10a-a"^^xsd:string ;
   rdf:type swrl:Imp ;
   swrl:body [ rdf:type swrl:AtomList ;
               rdf:first [ rdf:type swrl:IndividualPropertyAtom ;
                           swrl:propertyPredicate :has_SecuritySolution ;
                           swrl:argument1 <http://w3id.org/iot-tta#x> ;
                           swrl:argument2 <http://w3id.org/iot-tta#y>
                         ] ;
               rdf:rest [ rdf:type swrl:AtomList ;
                          rdf:first [ rdf:type swrl:ClassAtom ;
                                      swrl:classPredicate :Edge_security ;
                                      swrl:argument1 <http://w3id.org/iot-tta#x>
                                    ] ;
                          rdf:rest [ rdf:type swrl:AtomList ;
                                     rdf:first [ rdf:type swrl:ClassAtom ;
                                                 swrl:classPredicate :Blockchain_solution ;
                                                 swrl:argument1 <http://w3id.org/iot-tta#y>
                                               ] ;
                                     rdf:rest [ rdf:type swrl:AtomList ;
                                                rdf:first [ rdf:type swrl:IndividualPropertyAtom ;
                                                            swrl:propertyPredicate :best_Practices ;
                                                            swrl:argument1 <http://w3id.org/iot-tta#x> ;
                                                            swrl:argument2 <http://w3id.org/iot-tta#z>
                                                          ] ;
                                                rdf:rest rdf:nil
                                              ]
                                   ]
                        ]
             ] ;
   swrl:head [ rdf:type swrl:AtomList ;
               rdf:first [ rdf:type swrl:IndividualPropertyAtom ;
                           swrl:propertyPredicate :DevelopEdgeSecurity ;
                           swrl:argument1 <http://w3id.org/iot-tta#z> ;
                           swrl:argument2 <http://w3id.org/iot-tta#y>
                         ] ;
               rdf:rest rdf:nil
             ]
 ] .

[ swrla:isRuleEnabled "true"^^xsd:boolean ;
   rdfs:comment ""^^xsd:string ;
   rdfs:label "R10a-b"^^xsd:string ;
   rdf:type swrl:Imp ;
   swrl:body [ rdf:type swrl:AtomList ;
               rdf:first [ rdf:type swrl:IndividualPropertyAtom ;
                           swrl:propertyPredicate :has_SecuritySolution ;
                           swrl:argument1 <http://w3id.org/iot-tta#x> ;
                           swrl:argument2 <http://w3id.org/iot-tta#y>
                         ] ;
               rdf:rest [ rdf:type swrl:AtomList ;
                          rdf:first [ rdf:type swrl:ClassAtom ;
                                      swrl:classPredicate :Edge_security ;
                                      swrl:argument1 <http://w3id.org/iot-tta#x>
                                    ] ;
                          rdf:rest [ rdf:type swrl:AtomList ;
                                     rdf:first [ rdf:type swrl:ClassAtom ;
                                                 swrl:classPredicate :Blockchain_solution ;
                                                 swrl:argument1 <http://w3id.org/iot-tta#y>
                                               ] ;
                                     rdf:rest [ rdf:type swrl:AtomList ;
                                                rdf:first [ rdf:type swrl:IndividualPropertyAtom ;
                                                            swrl:propertyPredicate :best_Practices ;
                                                            swrl:argument1 <http://w3id.org/iot-tta#x> ;
                                                            swrl:argument2 <http://w3id.org/iot-tta#z>
                                                          ] ;
                                                rdf:rest rdf:nil
                                              ]
                                   ]
                        ]
             ] ;
   swrl:head [ rdf:type swrl:AtomList ;
               rdf:first [ rdf:type swrl:BuiltinAtom ;
                           swrl:builtin <http://sqwrl.stanford.edu/ontologies/built-ins/3.4/sqwrl.owl#select> ;
                           swrl:arguments ( <http://w3id.org/iot-tta#x>
                                            <http://w3id.org/iot-tta#y>
                                            <http://w3id.org/iot-tta#z>
                                          )
                         ] ;
               rdf:rest rdf:nil
             ]
 ] .

[ swrla:isRuleEnabled "true"^^xsd:boolean ;
   rdfs:comment ""^^xsd:string ;
   rdfs:label "R3s-b"^^xsd:string ;
   rdf:type swrl:Imp ;
   swrl:body [ rdf:type swrl:AtomList ;
               rdf:first [ rdf:type swrl:ClassAtom ;
                           swrl:classPredicate :Tool ;
                           swrl:argument1 :x
                         ] ;
               rdf:rest [ rdf:type swrl:AtomList ;
                          rdf:first [ rdf:type swrl:ClassAtom ;
                                      swrl:classPredicate :Computer_cluster ;
                                      swrl:argument1 :y
                                    ] ;
                          rdf:rest [ rdf:type swrl:AtomList ;
                                     rdf:first [ rdf:type swrl:IndividualPropertyAtom ;
                                                 swrl:propertyPredicate :useProgramming ;
                                                 swrl:argument1 :x ;
                                                 swrl:argument2 :z
                                               ] ;
                                     rdf:rest [ rdf:type swrl:AtomList ;
                                                rdf:first [ rdf:type swrl:IndividualPropertyAtom ;
                                                            swrl:propertyPredicate :isToolFor ;
                                                            swrl:argument1 :x ;
                                                            swrl:argument2 :y
                                                          ] ;
                                                rdf:rest rdf:nil
                                              ]
                                   ]
                        ]
             ] ;
   swrl:head [ rdf:type swrl:AtomList ;
               rdf:first [ rdf:type swrl:BuiltinAtom ;
                           swrl:builtin <http://sqwrl.stanford.edu/ontologies/built-ins/3.4/sqwrl.owl#select> ;
                           swrl:arguments ( :x
                                            :y
                                            :z
                                          )
                         ] ;
               rdf:rest rdf:nil
             ]
 ] .

[ swrla:isRuleEnabled "true"^^xsd:boolean ;
   rdfs:comment ""^^xsd:string ;
   rdfs:label "R2s-b"^^xsd:string ;
   rdf:type swrl:Imp ;
   swrl:body [ rdf:type swrl:AtomList ;
               rdf:first [ rdf:type swrl:IndividualPropertyAtom ;
                           swrl:propertyPredicate :useAlgorithm ;
                           swrl:argument1 <http://w3id.org/iot-tta#x> ;
                           swrl:argument2 <http://w3id.org/iot-tta#z>
                         ] ;
               rdf:rest [ rdf:type swrl:AtomList ;
                          rdf:first [ rdf:type swrl:IndividualPropertyAtom ;
                                      swrl:propertyPredicate :hasService ;
                                      swrl:argument1 <http://w3id.org/iot-tta#x> ;
                                      swrl:argument2 <http://w3id.org/iot-tta#y>
                                    ] ;
                          rdf:rest [ rdf:type swrl:AtomList ;
                                     rdf:first [ rdf:type swrl:ClassAtom ;
                                                 swrl:classPredicate :Data_center ;
                                                 swrl:argument1 <http://w3id.org/iot-tta#x>
                                               ] ;
                                     rdf:rest rdf:nil
                                   ]
                        ]
             ] ;
   swrl:head [ rdf:type swrl:AtomList ;
               rdf:first [ rdf:type swrl:BuiltinAtom ;
                           swrl:builtin <http://sqwrl.stanford.edu/ontologies/built-ins/3.4/sqwrl.owl#select> ;
                           swrl:arguments ( <http://w3id.org/iot-tta#x>
                                            <http://w3id.org/iot-tta#y>
                                            <http://w3id.org/iot-tta#z>
                                          )
                         ] ;
               rdf:rest rdf:nil
             ]
 ] .

[ swrla:isRuleEnabled "true"^^xsd:boolean ;
   rdfs:comment ""^^xsd:string ;
   rdfs:label "R2s-a"^^xsd:string ;
   rdf:type swrl:Imp ;
   swrl:body [ rdf:type swrl:AtomList ;
               rdf:first [ rdf:type swrl:IndividualPropertyAtom ;
                           swrl:propertyPredicate :useAlgorithm ;
                           swrl:argument1 <http://w3id.org/iot-tta/#x> ;
                           swrl:argument2 <http://w3id.org/iot-tta/#z>
                         ] ;
               rdf:rest [ rdf:type swrl:AtomList ;
                          rdf:first [ rdf:type swrl:ClassAtom ;
                                      swrl:classPredicate :Data_center ;
                                      swrl:argument1 <http://w3id.org/iot-tta/#x>
                                    ] ;
                          rdf:rest [ rdf:type swrl:AtomList ;
                                     rdf:first [ rdf:type swrl:IndividualPropertyAtom ;
                                                 swrl:propertyPredicate :hasService ;
                                                 swrl:argument1 <http://w3id.org/iot-tta/#x> ;
                                                 swrl:argument2 <http://w3id.org/iot-tta/#y>
                                               ] ;
                                     rdf:rest rdf:nil
                                   ]
                        ]
             ] ;
   swrl:head [ rdf:type swrl:AtomList ;
               rdf:first [ rdf:type swrl:IndividualPropertyAtom ;
                           swrl:propertyPredicate :hasFunctionality ;
                           swrl:argument1 <http://w3id.org/iot-tta/#x> ;
                           swrl:argument2 <http://w3id.org/iot-tta/#y>
                         ] ;
               rdf:rest rdf:nil
             ]
 ] .

[ swrla:isRuleEnabled "true"^^xsd:boolean ;
   rdfs:comment ""^^xsd:string ;
   rdfs:label "R11c-a"^^xsd:string ;
   rdf:type swrl:Imp ;
   swrl:body [ rdf:type swrl:AtomList ;
               rdf:first [ rdf:type swrl:ClassAtom ;
                           swrl:classPredicate :Flow ;
                           swrl:argument1 <http://w3id.org/iot-tta#y>
                         ] ;
               rdf:rest [ rdf:type swrl:AtomList ;
                          rdf:first [ rdf:type swrl:IndividualPropertyAtom ;
                                      swrl:propertyPredicate :send ;
                                      swrl:argument1 <http://w3id.org/iot-tta#z> ;
                                      swrl:argument2 <http://w3id.org/iot-tta#w>
                                    ] ;
                          rdf:rest [ rdf:type swrl:AtomList ;
                                     rdf:first [ rdf:type swrl:IndividualPropertyAtom ;
                                                 swrl:propertyPredicate :request ;
                                                 swrl:argument1 <http://w3id.org/iot-tta#w> ;
                                                 swrl:argument2 <http://w3id.org/iot-tta#q>
                                               ] ;
                                     rdf:rest [ rdf:type swrl:AtomList ;
                                                rdf:first [ rdf:type swrl:ClassAtom ;
                                                            swrl:classPredicate :Particle_cloud ;
                                                            swrl:argument1 <http://w3id.org/iot-tta#w>
                                                          ] ;
                                                rdf:rest [ rdf:type swrl:AtomList ;
                                                           rdf:first [ rdf:type swrl:DatavaluedPropertyAtom ;
                                                                       swrl:propertyPredicate :hasValueConnection ;
                                                                       swrl:argument1 <http://w3id.org/iot-tta#y> ;
                                                                       swrl:argument2 1
                                                                     ] ;
                                                           rdf:rest [ rdf:type swrl:AtomList ;
                                                                      rdf:first [ rdf:type swrl:ClassAtom ;
                                                                                  swrl:classPredicate :Firmware ;
                                                                                  swrl:argument1 <http://w3id.org/iot-tta#z>
                                                                                ] ;
                                                                      rdf:rest [ rdf:type swrl:AtomList ;
                                                                                 rdf:first [ rdf:type swrl:DatavaluedPropertyAtom ;
                                                                                             swrl:propertyPredicate :hasTimeLimit ;
                                                                                             swrl:argument1 <http://w3id.org/iot-tta#z> ;
                                                                                             swrl:argument2 30
                                                                                           ] ;
                                                                                 rdf:rest [ rdf:type swrl:AtomList ;
                                                                                            rdf:first [ rdf:type swrl:ClassAtom ;
                                                                                                        swrl:classPredicate :Subscriber ;
                                                                                                        swrl:argument1 <http://w3id.org/iot-tta#q>
                                                                                                      ] ;
                                                                                            rdf:rest [ rdf:type swrl:AtomList ;
                                                                                                       rdf:first [ rdf:type swrl:ClassAtom ;
                                                                                                                   swrl:classPredicate :Particle_Photon ;
                                                                                                                   swrl:argument1 <http://w3id.org/iot-tta#x>
                                                                                                                 ] ;
                                                                                                       rdf:rest [ rdf:type swrl:AtomList ;
                                                                                                                  rdf:first [ rdf:type swrl:IndividualPropertyAtom ;
                                                                                                                              swrl:propertyPredicate :read ;
                                                                                                                              swrl:argument1 <http://w3id.org/iot-tta#y> ;
                                                                                                                              swrl:argument2 <http://w3id.org/iot-tta#z>
                                                                                                                            ] ;
                                                                                                                  rdf:rest [ rdf:type swrl:AtomList ;
                                                                                                                             rdf:first [ rdf:type swrl:IndividualPropertyAtom ;
                                                                                                                                         swrl:propertyPredicate :wire ;
                                                                                                                                         swrl:argument1 <http://w3id.org/iot-tta#x> ;
                                                                                                                                         swrl:argument2 <http://w3id.org/iot-tta#y>
                                                                                                                                       ] ;
                                                                                                                             rdf:rest rdf:nil
                                                                                                                           ]
                                                                                                                ]
                                                                                                     ]
                                                                                          ]
                                                                               ]
                                                                    ]
                                                         ]
                                              ]
                                   ]
                        ]
             ] ;
   swrl:head [ rdf:type swrl:AtomList ;
               rdf:first [ rdf:type swrl:IndividualPropertyAtom ;
                           swrl:propertyPredicate :flow_services ;
                           swrl:argument1 <http://w3id.org/iot-tta#x> ;
                           swrl:argument2 <http://w3id.org/iot-tta#q>
                         ] ;
               rdf:rest rdf:nil
             ]
 ] .

[ swrla:isRuleEnabled "true"^^xsd:boolean ;
   rdfs:comment ""^^xsd:string ;
   rdfs:label "R11c-b"^^xsd:string ;
   rdf:type swrl:Imp ;
   swrl:body [ rdf:type swrl:AtomList ;
               rdf:first [ rdf:type swrl:ClassAtom ;
                           swrl:classPredicate :Flow ;
                           swrl:argument1 <http://w3id.org/iot-tta#y>
                         ] ;
               rdf:rest [ rdf:type swrl:AtomList ;
                          rdf:first [ rdf:type swrl:IndividualPropertyAtom ;
                                      swrl:propertyPredicate :send ;
                                      swrl:argument1 <http://w3id.org/iot-tta#z> ;
                                      swrl:argument2 <http://w3id.org/iot-tta#w>
                                    ] ;
                          rdf:rest [ rdf:type swrl:AtomList ;
                                     rdf:first [ rdf:type swrl:IndividualPropertyAtom ;
                                                 swrl:propertyPredicate :request ;
                                                 swrl:argument1 <http://w3id.org/iot-tta#w> ;
                                                 swrl:argument2 <http://w3id.org/iot-tta#q>
                                               ] ;
                                     rdf:rest [ rdf:type swrl:AtomList ;
                                                rdf:first [ rdf:type swrl:ClassAtom ;
                                                            swrl:classPredicate :Particle_cloud ;
                                                            swrl:argument1 <http://w3id.org/iot-tta#w>
                                                          ] ;
                                                rdf:rest [ rdf:type swrl:AtomList ;
                                                           rdf:first [ rdf:type swrl:DatavaluedPropertyAtom ;
                                                                       swrl:propertyPredicate :hasValueConnection ;
                                                                       swrl:argument1 <http://w3id.org/iot-tta#y> ;
                                                                       swrl:argument2 1
                                                                     ] ;
                                                           rdf:rest [ rdf:type swrl:AtomList ;
                                                                      rdf:first [ rdf:type swrl:ClassAtom ;
                                                                                  swrl:classPredicate :Firmware ;
                                                                                  swrl:argument1 <http://w3id.org/iot-tta#z>
                                                                                ] ;
                                                                      rdf:rest [ rdf:type swrl:AtomList ;
                                                                                 rdf:first [ rdf:type swrl:DatavaluedPropertyAtom ;
                                                                                             swrl:propertyPredicate :hasTimeLimit ;
                                                                                             swrl:argument1 <http://w3id.org/iot-tta#z> ;
                                                                                             swrl:argument2 30
                                                                                           ] ;
                                                                                 rdf:rest [ rdf:type swrl:AtomList ;
                                                                                            rdf:first [ rdf:type swrl:ClassAtom ;
                                                                                                        swrl:classPredicate :Subscriber ;
                                                                                                        swrl:argument1 <http://w3id.org/iot-tta#q>
                                                                                                      ] ;
                                                                                            rdf:rest [ rdf:type swrl:AtomList ;
                                                                                                       rdf:first [ rdf:type swrl:ClassAtom ;
                                                                                                                   swrl:classPredicate :Particle_Photon ;
                                                                                                                   swrl:argument1 <http://w3id.org/iot-tta#x>
                                                                                                                 ] ;
                                                                                                       rdf:rest [ rdf:type swrl:AtomList ;
                                                                                                                  rdf:first [ rdf:type swrl:IndividualPropertyAtom ;
                                                                                                                              swrl:propertyPredicate :read ;
                                                                                                                              swrl:argument1 <http://w3id.org/iot-tta#y> ;
                                                                                                                              swrl:argument2 <http://w3id.org/iot-tta#z>
                                                                                                                            ] ;
                                                                                                                  rdf:rest [ rdf:type swrl:AtomList ;
                                                                                                                             rdf:first [ rdf:type swrl:IndividualPropertyAtom ;
                                                                                                                                         swrl:propertyPredicate :wire ;
                                                                                                                                         swrl:argument1 <http://w3id.org/iot-tta#x> ;
                                                                                                                                         swrl:argument2 <http://w3id.org/iot-tta#y>
                                                                                                                                       ] ;
                                                                                                                             rdf:rest rdf:nil
                                                                                                                           ]
                                                                                                                ]
                                                                                                     ]
                                                                                          ]
                                                                               ]
                                                                    ]
                                                         ]
                                              ]
                                   ]
                        ]
             ] ;
   swrl:head [ rdf:type swrl:AtomList ;
               rdf:first [ rdf:type swrl:BuiltinAtom ;
                           swrl:builtin <http://sqwrl.stanford.edu/ontologies/built-ins/3.4/sqwrl.owl#select> ;
                           swrl:arguments ( <http://w3id.org/iot-tta#x>
                                            <http://w3id.org/iot-tta#y>
                                            <http://w3id.org/iot-tta#z>
                                            <http://w3id.org/iot-tta#w>
                                            <http://w3id.org/iot-tta#q>
                                          )
                         ] ;
               rdf:rest rdf:nil
             ]
 ] .

[ swrla:isRuleEnabled "true"^^xsd:boolean ;
   rdfs:comment ""^^xsd:string ;
   rdfs:label "R12c-a"^^xsd:string ;
   rdf:type swrl:Imp ;
   swrl:body [ rdf:type swrl:AtomList ;
               rdf:first [ rdf:type swrl:ClassAtom ;
                           swrl:classPredicate :RTD_sensor ;
                           swrl:argument1 <http://w3id.org/iot-tta#x>
                         ] ;
               rdf:rest [ rdf:type swrl:AtomList ;
                          rdf:first [ rdf:type swrl:DatavaluedPropertyAtom ;
                                      swrl:propertyPredicate :provideHeat ;
                                      swrl:argument1 <http://w3id.org/iot-tta#x> ;
                                      swrl:argument2 <http://w3id.org/iot-tta#z>
                                    ] ;
                          rdf:rest [ rdf:type swrl:AtomList ;
                                     rdf:first [ rdf:type swrl:DatavaluedPropertyAtom ;
                                                 swrl:propertyPredicate :hasAccuracy ;
                                                 swrl:argument1 <http://w3id.org/iot-tta#x> ;
                                                 swrl:argument2 <http://w3id.org/iot-tta#t>
                                               ] ;
                                     rdf:rest [ rdf:type swrl:AtomList ;
                                                rdf:first [ rdf:type swrl:DatavaluedPropertyAtom ;
                                                            swrl:propertyPredicate :hasTemperatureRange ;
                                                            swrl:argument1 <http://w3id.org/iot-tta#y> ;
                                                            swrl:argument2 <http://w3id.org/iot-tta#w>
                                                          ] ;
                                                rdf:rest [ rdf:type swrl:AtomList ;
                                                           rdf:first [ rdf:type swrl:BuiltinAtom ;
                                                                       swrl:builtin swrlb:greaterThan ;
                                                                       swrl:arguments ( <http://w3id.org/iot-tta#z>
                                                                                        <http://w3id.org/iot-tta#w>
                                                                                      )
                                                                     ] ;
                                                           rdf:rest [ rdf:type swrl:AtomList ;
                                                                      rdf:first [ rdf:type swrl:BuiltinAtom ;
                                                                                  swrl:builtin swrlb:greaterThan ;
                                                                                  swrl:arguments [ rdf:type rdf:List ;
                                                                                                   rdf:first <http://w3id.org/iot-tta#t> ;
                                                                                                   rdf:rest [ rdf:type rdf:List ;
                                                                                                              rdf:first 0.7 ;
                                                                                                              rdf:rest rdf:nil
                                                                                                            ]
                                                                                                 ]
                                                                                ] ;
                                                                      rdf:rest [ rdf:type swrl:AtomList ;
                                                                                 rdf:first [ rdf:type swrl:IndividualPropertyAtom ;
                                                                                             swrl:propertyPredicate :heat ;
                                                                                             swrl:argument1 <http://w3id.org/iot-tta#x> ;
                                                                                             swrl:argument2 <http://w3id.org/iot-tta#y>
                                                                                           ] ;
                                                                                 rdf:rest [ rdf:type swrl:AtomList ;
                                                                                            rdf:first [ rdf:type swrl:ClassAtom ;
                                                                                                        swrl:classPredicate :Industrial_oven ;
                                                                                                        swrl:argument1 <http://w3id.org/iot-tta#y>
                                                                                                      ] ;
                                                                                            rdf:rest rdf:nil
                                                                                          ]
                                                                               ]
                                                                    ]
                                                         ]
                                              ]
                                   ]
                        ]
             ] ;
   swrl:head [ rdf:type swrl:AtomList ;
               rdf:first [ rdf:type swrl:IndividualPropertyAtom ;
                           swrl:propertyPredicate :regulationTemperature ;
                           swrl:argument1 <http://w3id.org/iot-tta#x> ;
                           swrl:argument2 <http://w3id.org/iot-tta#y>
                         ] ;
               rdf:rest rdf:nil
             ]
 ] .

[ swrla:isRuleEnabled "true"^^xsd:boolean ;
   rdfs:comment ""^^xsd:string ;
   rdfs:label "R12c-b"^^xsd:string ;
   rdf:type swrl:Imp ;
   swrl:body [ rdf:type swrl:AtomList ;
               rdf:first [ rdf:type swrl:ClassAtom ;
                           swrl:classPredicate :RTD_sensor ;
                           swrl:argument1 <http://w3id.org/iot-tta#x>
                         ] ;
               rdf:rest [ rdf:type swrl:AtomList ;
                          rdf:first [ rdf:type swrl:DatavaluedPropertyAtom ;
                                      swrl:propertyPredicate :provideHeat ;
                                      swrl:argument1 <http://w3id.org/iot-tta#x> ;
                                      swrl:argument2 <http://w3id.org/iot-tta#z>
                                    ] ;
                          rdf:rest [ rdf:type swrl:AtomList ;
                                     rdf:first [ rdf:type swrl:DatavaluedPropertyAtom ;
                                                 swrl:propertyPredicate :hasAccuracy ;
                                                 swrl:argument1 <http://w3id.org/iot-tta#x> ;
                                                 swrl:argument2 <http://w3id.org/iot-tta#t>
                                               ] ;
                                     rdf:rest [ rdf:type swrl:AtomList ;
                                                rdf:first [ rdf:type swrl:DatavaluedPropertyAtom ;
                                                            swrl:propertyPredicate :hasTemperatureRange ;
                                                            swrl:argument1 <http://w3id.org/iot-tta#y> ;
                                                            swrl:argument2 <http://w3id.org/iot-tta#w>
                                                          ] ;
                                                rdf:rest [ rdf:type swrl:AtomList ;
                                                           rdf:first [ rdf:type swrl:BuiltinAtom ;
                                                                       swrl:builtin swrlb:greaterThan ;
                                                                       swrl:arguments ( <http://w3id.org/iot-tta#z>
                                                                                        <http://w3id.org/iot-tta#w>
                                                                                      )
                                                                     ] ;
                                                           rdf:rest [ rdf:type swrl:AtomList ;
                                                                      rdf:first [ rdf:type swrl:BuiltinAtom ;
                                                                                  swrl:builtin swrlb:greaterThan ;
                                                                                  swrl:arguments [ rdf:type rdf:List ;
                                                                                                   rdf:first <http://w3id.org/iot-tta#t> ;
                                                                                                   rdf:rest [ rdf:type rdf:List ;
                                                                                                              rdf:first 0.7 ;
                                                                                                              rdf:rest rdf:nil
                                                                                                            ]
                                                                                                 ]
                                                                                ] ;
                                                                      rdf:rest [ rdf:type swrl:AtomList ;
                                                                                 rdf:first [ rdf:type swrl:IndividualPropertyAtom ;
                                                                                             swrl:propertyPredicate :heat ;
                                                                                             swrl:argument1 <http://w3id.org/iot-tta#x> ;
                                                                                             swrl:argument2 <http://w3id.org/iot-tta#y>
                                                                                           ] ;
                                                                                 rdf:rest [ rdf:type swrl:AtomList ;
                                                                                            rdf:first [ rdf:type swrl:ClassAtom ;
                                                                                                        swrl:classPredicate :Industrial_oven ;
                                                                                                        swrl:argument1 <http://w3id.org/iot-tta#y>
                                                                                                      ] ;
                                                                                            rdf:rest rdf:nil
                                                                                          ]
                                                                               ]
                                                                    ]
                                                         ]
                                              ]
                                   ]
                        ]
             ] ;
   swrl:head [ rdf:type swrl:AtomList ;
               rdf:first [ rdf:type swrl:BuiltinAtom ;
                           swrl:builtin <http://sqwrl.stanford.edu/ontologies/built-ins/3.4/sqwrl.owl#select> ;
                           swrl:arguments ( <http://w3id.org/iot-tta#x>
                                            <http://w3id.org/iot-tta#z>
                                            <http://w3id.org/iot-tta#y>
                                            <http://w3id.org/iot-tta#w>
                                            <http://w3id.org/iot-tta#t>
                                          )
                         ] ;
               rdf:rest rdf:nil
             ]
 ] .

[ swrla:isRuleEnabled "true"^^xsd:boolean ;
   rdfs:comment ""^^xsd:string ;
   rdfs:label "R7a-b"^^xsd:string ;
   rdf:type swrl:Imp ;
   swrl:body [ rdf:type swrl:AtomList ;
               rdf:first [ rdf:type swrl:IndividualPropertyAtom ;
                           swrl:propertyPredicate :Lack_security_measure ;
                           swrl:argument1 <http://w3id.org/iot-tta#x> ;
                           swrl:argument2 <http://w3id.org/iot-tta#y>
                         ] ;
               rdf:rest [ rdf:type swrl:AtomList ;
                          rdf:first [ rdf:type swrl:IndividualPropertyAtom ;
                                      swrl:propertyPredicate :Protocols_were_layered ;
                                      swrl:argument1 <http://w3id.org/iot-tta#x> ;
                                      swrl:argument2 <http://w3id.org/iot-tta#z>
                                    ] ;
                          rdf:rest [ rdf:type swrl:AtomList ;
                                     rdf:first [ rdf:type swrl:IndividualPropertyAtom ;
                                                 swrl:propertyPredicate :Support_communication ;
                                                 swrl:argument1 <http://w3id.org/iot-tta#z> ;
                                                 swrl:argument2 <http://w3id.org/iot-tta#w>
                                               ] ;
                                     rdf:rest [ rdf:type swrl:AtomList ;
                                                rdf:first [ rdf:type swrl:IndividualPropertyAtom ;
                                                            swrl:propertyPredicate :SCADA_hasCapability ;
                                                            swrl:argument1 <http://w3id.org/iot-tta#s> ;
                                                            swrl:argument2 <http://w3id.org/iot-tta#w>
                                                          ] ;
                                                rdf:rest [ rdf:type swrl:AtomList ;
                                                           rdf:first [ rdf:type swrl:ClassAtom ;
                                                                       swrl:classPredicate :SCADA ;
                                                                       swrl:argument1 <http://w3id.org/iot-tta#s>
                                                                     ] ;
                                                           rdf:rest rdf:nil
                                                         ]
                                              ]
                                   ]
                        ]
             ] ;
   swrl:head [ rdf:type swrl:AtomList ;
               rdf:first [ rdf:type swrl:BuiltinAtom ;
                           swrl:builtin <http://sqwrl.stanford.edu/ontologies/built-ins/3.4/sqwrl.owl#select> ;
                           swrl:arguments ( <http://w3id.org/iot-tta#s>
                                            <http://w3id.org/iot-tta#x>
                                            <http://w3id.org/iot-tta#y>
                                            <http://w3id.org/iot-tta#z>
                                            <http://w3id.org/iot-tta#w>
                                          )
                         ] ;
               rdf:rest rdf:nil
             ]
 ] .

[ swrla:isRuleEnabled "true"^^xsd:boolean ;
   rdfs:comment ""^^xsd:string ;
   rdfs:label "R7a-a"^^xsd:string ;
   rdf:type swrl:Imp ;
   swrl:body [ rdf:type swrl:AtomList ;
               rdf:first [ rdf:type swrl:IndividualPropertyAtom ;
                           swrl:propertyPredicate :Lack_security_measure ;
                           swrl:argument1 <http://w3id.org/iot-tta#x> ;
                           swrl:argument2 <http://w3id.org/iot-tta#y>
                         ] ;
               rdf:rest [ rdf:type swrl:AtomList ;
                          rdf:first [ rdf:type swrl:IndividualPropertyAtom ;
                                      swrl:propertyPredicate :Protocols_were_layered ;
                                      swrl:argument1 <http://w3id.org/iot-tta#x> ;
                                      swrl:argument2 <http://w3id.org/iot-tta#z>
                                    ] ;
                          rdf:rest [ rdf:type swrl:AtomList ;
                                     rdf:first [ rdf:type swrl:IndividualPropertyAtom ;
                                                 swrl:propertyPredicate :Support_communication ;
                                                 swrl:argument1 <http://w3id.org/iot-tta#z> ;
                                                 swrl:argument2 <http://w3id.org/iot-tta#w>
                                               ] ;
                                     rdf:rest [ rdf:type swrl:AtomList ;
                                                rdf:first [ rdf:type swrl:ClassAtom ;
                                                            swrl:classPredicate :SCADA ;
                                                            swrl:argument1 <http://w3id.org/iot-tta#s>
                                                          ] ;
                                                rdf:rest rdf:nil
                                              ]
                                   ]
                        ]
             ] ;
   swrl:head [ rdf:type swrl:AtomList ;
               rdf:first [ rdf:type swrl:IndividualPropertyAtom ;
                           swrl:propertyPredicate :SCADA_hasCapability ;
                           swrl:argument1 <http://w3id.org/iot-tta#s> ;
                           swrl:argument2 <http://w3id.org/iot-tta#w>
                         ] ;
               rdf:rest rdf:nil
             ]
 ] .

[ swrla:isRuleEnabled "true"^^xsd:boolean ;
   rdfs:comment ""^^xsd:string ;
   rdfs:label "R8a-a"^^xsd:string ;
   rdf:type swrl:Imp ;
   swrl:body [ rdf:type swrl:AtomList ;
               rdf:first [ rdf:type swrl:ClassAtom ;
                           swrl:classPredicate :SCADA ;
                           swrl:argument1 <http://w3id.org/iot-tta#x>
                         ] ;
               rdf:rest [ rdf:type swrl:AtomList ;
                          rdf:first [ rdf:type swrl:IndividualPropertyAtom ;
                                      swrl:propertyPredicate :countermeasure ;
                                      swrl:argument1 <http://w3id.org/iot-tta#y> ;
                                      swrl:argument2 <http://w3id.org/iot-tta#z>
                                    ] ;
                          rdf:rest [ rdf:type swrl:AtomList ;
                                     rdf:first [ rdf:type swrl:IndividualPropertyAtom ;
                                                 swrl:propertyPredicate :threats_to_data_security ;
                                                 swrl:argument1 <http://w3id.org/iot-tta#x> ;
                                                 swrl:argument2 <http://w3id.org/iot-tta#y>
                                               ] ;
                                     rdf:rest rdf:nil
                                   ]
                        ]
             ] ;
   swrl:head [ rdf:type swrl:AtomList ;
               rdf:first [ rdf:type swrl:IndividualPropertyAtom ;
                           swrl:propertyPredicate :Dealing_with_sensitive_data ;
                           swrl:argument1 <http://w3id.org/iot-tta#x> ;
                           swrl:argument2 <http://w3id.org/iot-tta#z>
                         ] ;
               rdf:rest rdf:nil
             ]
 ] .

[ swrla:isRuleEnabled "true"^^xsd:boolean ;
   rdfs:comment ""^^xsd:string ;
   rdfs:label "R8a-b"^^xsd:string ;
   rdf:type swrl:Imp ;
   swrl:body [ rdf:type swrl:AtomList ;
               rdf:first [ rdf:type swrl:ClassAtom ;
                           swrl:classPredicate :SCADA ;
                           swrl:argument1 <http://w3id.org/iot-tta#x>
                         ] ;
               rdf:rest [ rdf:type swrl:AtomList ;
                          rdf:first [ rdf:type swrl:IndividualPropertyAtom ;
                                      swrl:propertyPredicate :countermeasure ;
                                      swrl:argument1 <http://w3id.org/iot-tta#y> ;
                                      swrl:argument2 <http://w3id.org/iot-tta#z>
                                    ] ;
                          rdf:rest [ rdf:type swrl:AtomList ;
                                     rdf:first [ rdf:type swrl:IndividualPropertyAtom ;
                                                 swrl:propertyPredicate :threats_to_data_security ;
                                                 swrl:argument1 <http://w3id.org/iot-tta#x> ;
                                                 swrl:argument2 <http://w3id.org/iot-tta#y>
                                               ] ;
                                     rdf:rest rdf:nil
                                   ]
                        ]
             ] ;
   swrl:head [ rdf:type swrl:AtomList ;
               rdf:first [ rdf:type swrl:BuiltinAtom ;
                           swrl:builtin <http://sqwrl.stanford.edu/ontologies/built-ins/3.4/sqwrl.owl#select> ;
                           swrl:arguments ( <http://w3id.org/iot-tta#x>
                                            <http://w3id.org/iot-tta#y>
                                            <http://w3id.org/iot-tta#z>
                                          )
                         ] ;
               rdf:rest rdf:nil
             ]
 ] .

[ swrla:isRuleEnabled "true"^^xsd:boolean ;
   rdfs:comment ""^^xsd:string ;
   rdfs:label "R1s-b"^^xsd:string ;
   rdf:type swrl:Imp ;
   swrl:body [ rdf:type swrl:AtomList ;
               rdf:first [ rdf:type swrl:IndividualPropertyAtom ;
                           swrl:propertyPredicate :isToolFor ;
                           swrl:argument1 :y ;
                           swrl:argument2 :x
                         ] ;
               rdf:rest [ rdf:type swrl:AtomList ;
                          rdf:first [ rdf:type swrl:ClassAtom ;
                                      swrl:classPredicate :Technology ;
                                      swrl:argument1 :Deep_learning_algorithm
                                    ] ;
                          rdf:rest [ rdf:type swrl:AtomList ;
                                     rdf:first [ rdf:type swrl:IndividualPropertyAtom ;
                                                 swrl:propertyPredicate :hasTool ;
                                                 swrl:argument1 :x ;
                                                 swrl:argument2 :y
                                               ] ;
                                     rdf:rest rdf:nil
                                   ]
                        ]
             ] ;
   swrl:head [ rdf:type swrl:AtomList ;
               rdf:first [ rdf:type swrl:BuiltinAtom ;
                           swrl:builtin <http://sqwrl.stanford.edu/ontologies/built-ins/3.4/sqwrl.owl#select> ;
                           swrl:arguments ( :x
                                            :y
                                          )
                         ] ;
               rdf:rest rdf:nil
             ]
 ] .

[ swrla:isRuleEnabled "true"^^xsd:boolean ;
   rdfs:comment ""^^xsd:string ;
   rdfs:label "R1s-a"^^xsd:string ;
   rdf:type swrl:Imp ;
   swrl:body [ rdf:type swrl:AtomList ;
               rdf:first [ rdf:type swrl:IndividualPropertyAtom ;
                           swrl:propertyPredicate :isToolFor ;
                           swrl:argument1 :z ;
                           swrl:argument2 :x
                         ] ;
               rdf:rest [ rdf:type swrl:AtomList ;
                          rdf:first [ rdf:type swrl:ClassAtom ;
                                      swrl:classPredicate :Technology ;
                                      swrl:argument1 :Deep_learning_algorithm
                                    ] ;
                          rdf:rest [ rdf:type swrl:AtomList ;
                                     rdf:first [ rdf:type swrl:IndividualPropertyAtom ;
                                                 swrl:propertyPredicate :hasTool ;
                                                 swrl:argument1 :x ;
                                                 swrl:argument2 :y
                                               ] ;
                                     rdf:rest rdf:nil
                                   ]
                        ]
             ] ;
   swrl:head [ rdf:type swrl:AtomList ;
               rdf:first [ rdf:type swrl:IndividualPropertyAtom ;
                           swrl:propertyPredicate :isToolFor ;
                           swrl:argument1 :y ;
                           swrl:argument2 :x
                         ] ;
               rdf:rest [ rdf:type swrl:AtomList ;
                          rdf:first [ rdf:type swrl:IndividualPropertyAtom ;
                                      swrl:propertyPredicate :hasTool ;
                                      swrl:argument1 :x ;
                                      swrl:argument2 :z
                                    ] ;
                          rdf:rest rdf:nil
                        ]
             ]
 ] .

[ swrla:isRuleEnabled "true"^^xsd:boolean ;
   rdfs:comment ""^^xsd:string ;
   rdfs:label "R3s-a"^^xsd:string ;
   rdf:type swrl:Imp ;
   swrl:body [ rdf:type swrl:AtomList ;
               rdf:first [ rdf:type swrl:IndividualPropertyAtom ;
                           swrl:propertyPredicate :isApplied ;
                           swrl:argument1 :z ;
                           swrl:argument2 :y
                         ] ;
               rdf:rest [ rdf:type swrl:AtomList ;
                          rdf:first [ rdf:type swrl:IndividualPropertyAtom ;
                                      swrl:propertyPredicate :isUsedBy ;
                                      swrl:argument1 :x ;
                                      swrl:argument2 :y
                                    ] ;
                          rdf:rest [ rdf:type swrl:AtomList ;
                                     rdf:first [ rdf:type swrl:ClassAtom ;
                                                 swrl:classPredicate :Tool ;
                                                 swrl:argument1 :Hadoop
                                               ] ;
                                     rdf:rest rdf:nil
                                   ]
                        ]
             ] ;
   swrl:head [ rdf:type swrl:AtomList ;
               rdf:first [ rdf:type swrl:IndividualPropertyAtom ;
                           swrl:propertyPredicate :isToolFor ;
                           swrl:argument1 :x ;
                           swrl:argument2 :y
                         ] ;
               rdf:rest [ rdf:type swrl:AtomList ;
                          rdf:first [ rdf:type swrl:IndividualPropertyAtom ;
                                      swrl:propertyPredicate :useProgramming ;
                                      swrl:argument1 :x ;
                                      swrl:argument2 :z
                                    ] ;
                          rdf:rest rdf:nil
                        ]
             ]
 ] .

###  Generated by the OWL API (version 4.5.9.2019-02-01T07:24:44Z) https://github.com/owlcs/owlapi
